instantiation/MemoryInvariant.thy
@@ -19,7 +19,7 @@ abbreviation (out) MemoryInvariantPost where
   "MemoryInvariantPost addr val \<equiv> 
    read_state getExceptionSignalled \<or>\<^sub>b
    read_state isUnpredictable \<or>\<^sub>b
-   (read_state (getMemData addr) =\<^sub>b return val)"
+   (read_state (getMemByte addr) =\<^sub>b return val)"
   
 method MemoryInvariant uses intro =
   PrePost intro: intro MemoryInvariantI[THEN PrePost_post_weakening]
@@ -35,13 +35,13 @@ method MemoryInvariant uses intro =
 (* Code generation - skip - SignalCapException_noReg *)
 
 lemma MemoryInvariant_dfn'ERET [MemoryInvariantI]:
-  shows "PrePost ((read_state (getMemData a) =\<^sub>b return val) \<and>\<^sub>b
+  shows "PrePost ((read_state (getMemByte a) =\<^sub>b return val) \<and>\<^sub>b
                   bind ERETActions
                        (\<lambda>p. return (a \<notin> \<Union> (WrittenAddresses ` p))))
                  dfn'ERET
                  (\<lambda>_. read_state getExceptionSignalled \<or>\<^sub>b
                       read_state isUnpredictable \<or>\<^sub>b
-                      read_state (getMemData a) =\<^sub>b return val)"
+                      read_state (getMemByte a) =\<^sub>b return val)"
 unfolding dfn'ERET_alt_def ERETActions_def 
 unfolding LegacyStoreActions_def LegacyStorePhysicalAddress_def LegacyStoreVirtualAddress_def
 unfolding BYTE_def HALFWORD_def WORD_def DOUBLEWORD_def
@@ -69,15 +69,15 @@ using assms
 unfolding extract_byte_updateDwordInRaw
 by auto
 
-lemma MemoryInvariant_WriteData_getMemData:
+lemma MemoryInvariant_WriteData_getMemByte:
   assumes "slice 3 addr = addr' \<Longrightarrow> extract_byte (unat (addr XOR mask 3) mod 8) msk = 0"
-  shows "IsInvariant (read_state (getMemData addr) =\<^sub>b return val)
+  shows "IsInvariant (read_state (getMemByte addr) =\<^sub>b return val)
                      (WriteData (addr', val', msk))"
 proof (cases "(slice 5 addr::35 word) = slice 2 addr'")
   case False
   show ?thesis
     unfolding WriteData_alt_def write'MEM_alt_def 
-    by PrePost (auto simp: getMemData_def Let_def MEM_def ValuePart_bind ucast_shiftr False)
+    by PrePost (auto simp: getMemByte_def Let_def MEM_def ValuePart_bind ucast_shiftr False)
 next
   case True
   have "(8::nat) dvd 32" by arith
@@ -131,7 +131,7 @@ next
     by (intro updateDwordInRaw_idem) auto
   show ?thesis
     unfolding WriteData_alt_def write'MEM_alt_def 
-    by PrePost (auto simp: getMemData_def Let_def MEM_def ValuePart_bind ucast_shiftr)
+    by PrePost (auto simp: getMemByte_def Let_def MEM_def ValuePart_bind ucast_shiftr)
 qed
 
 (* We deliberately don't add the lemma to MemoryInvariantI. *)
@@ -140,9 +140,9 @@ lemma MemoryInvariant_WriteData:
   shows "PrePost (return (case v of (addr', val', msk) \<Rightarrow>
                           slice 3 a \<noteq> addr' \<or>
                           extract_byte (unat (a XOR mask 3) mod 8) msk = 0) \<and>\<^sub>b
-                  (read_state (getMemData a) =\<^sub>b return val)) 
+                  (read_state (getMemByte a) =\<^sub>b return val)) 
                  (WriteData v)
-                 (\<lambda>_. read_state (getMemData a) =\<^sub>b return val)" 
+                 (\<lambda>_. read_state (getMemByte a) =\<^sub>b return val)" 
   (is "PrePost ?p ?m ?q")
 proof (intro PrePostI)
   fix s
@@ -151,11 +151,11 @@ proof (intro PrePostI)
   if "slice 3 a = fst v"
     using as that
     by (cases v) (strong_cong_simp add: ValueAndStatePart_simp if_bool_simps)
-  note aux = MemoryInvariant_WriteData_getMemData[OF this]
-  have "ValuePart (read_state (getMemData a) =\<^sub>b return val) s"
+  note aux = MemoryInvariant_WriteData_getMemByte[OF this]
+  have "ValuePart (read_state (getMemByte a) =\<^sub>b return val) s"
     using as by (auto simp: ValueAndStatePart_simp)
   note PrePostE[where s=s, OF aux this]
-  thus "ValuePart (bind (WriteData v) (\<lambda>_. read_state (getMemData a) =\<^sub>b return val)) s"
+  thus "ValuePart (bind (WriteData v) (\<lambda>_. read_state (getMemByte a) =\<^sub>b return val)) s"
     by (cases v) (simp add: ValueAndStatePart_simp)
 qed
 
@@ -165,16 +165,16 @@ qed
 
 lemma MemoryInvariant_WriteCap_aux2:
   assumes "slice (log2 CAPBYTEWIDTH) addr \<noteq> addr'"
-  shows "getMemData addr (setMEM (v, addr') s) = getMemData addr s" 
+  shows "getMemByte addr (setMEM (v, addr') s) = getMemByte addr s" 
 using assms
-unfolding getMemData_def Let_def
+unfolding getMemByte_def Let_def
 by auto
 
 lemma MemoryInvariant_WriteCap_aux:
   shows "PrePost (return (slice (log2 CAPBYTEWIDTH) addr \<noteq> fst v) \<and>\<^sub>b
-                  (read_state (getMemData addr) =\<^sub>b return val)) 
+                  (read_state (getMemByte addr) =\<^sub>b return val)) 
                  (WriteCap v)
-                 (\<lambda>_. read_state (getMemData addr) =\<^sub>b return val)"
+                 (\<lambda>_. read_state (getMemByte addr) =\<^sub>b return val)"
 unfolding WriteCap_alt_def 
 by PrePost (auto intro!: MemoryInvariant_WriteCap_aux2)
 
@@ -191,15 +191,15 @@ lemmas MemoryInvariant_WriteCap [MemoryInvariantI] =
 (* Code generation - end override *)
 
 lemma MemoryInvariant_LoadMemoryCap [MemoryInvariantI]:
-  shows "IsInvariant (read_state (getMemData a) =\<^sub>b return val) (LoadMemoryCap v)"
+  shows "IsInvariant (read_state (getMemByte a) =\<^sub>b return val) (LoadMemoryCap v)"
 by MemoryInvariant auto?
 
 lemma MemoryInvariant_LoadMemory [MemoryInvariantI]:
-  shows "IsInvariant (read_state (getMemData a) =\<^sub>b return val) (LoadMemory v)"
+  shows "IsInvariant (read_state (getMemByte a) =\<^sub>b return val) (LoadMemory v)"
 by MemoryInvariant auto?
 
 lemma MemoryInvariant_LoadCap [MemoryInvariantI]:
-  shows "IsInvariant (read_state (getMemData a) =\<^sub>b return val) (LoadCap v)"
+  shows "IsInvariant (read_state (getMemByte a) =\<^sub>b return val) (LoadCap v)"
 by MemoryInvariant auto?
 
 (* Code generation - override - StoreMemoryCap *)
@@ -289,9 +289,9 @@ lemma MemoryInvariant_WriteData_specific_Mem:
                           ((unat length + unat vAddr' mod 8 < unat addr mod 8 \<or> 
                             unat addr mod 8 < unat vAddr' mod 8) \<and>
                            unat vAddr' mod 8 + unat length < 8)) \<and>\<^sub>b
-                  (read_state (getMemData addr) =\<^sub>b return val))
+                  (read_state (getMemByte addr) =\<^sub>b return val))
                  (WriteData (slice 3 addr', x, (2 ^ m - 2 ^ n)))
-                 (\<lambda>_. read_state (getMemData addr) =\<^sub>b return val)"
+                 (\<lambda>_. read_state (getMemByte addr) =\<^sub>b return val)"
 unfolding m_def n_def
 using extract_byte_from_WriteData_mask
 by (intro PrePostIE[OF MemoryInvariant_WriteData])
@@ -316,12 +316,12 @@ lemma MemoryInvariant_AdjustEndian [MemoryInvariantI]:
   shows "PrePost (read_state getExceptionSignalled \<or>\<^sub>b
                   read_state isUnpredictable \<or>\<^sub>b
                   (return ((slice 3 a::37 word) \<noteq> slice 3 (snd v) \<or> b) \<and>\<^sub>b 
-                   (read_state (getMemData a) =\<^sub>b return val)))
+                   (read_state (getMemByte a) =\<^sub>b return val)))
                  (AdjustEndian v)
                  (\<lambda>x. read_state getExceptionSignalled \<or>\<^sub>b
                       read_state isUnpredictable \<or>\<^sub>b
                       (return ((slice 3 a::37 word) \<noteq> slice 3 x \<or> b) \<and>\<^sub>b 
-                       (read_state (getMemData a) =\<^sub>b return val)))"
+                       (read_state (getMemByte a) =\<^sub>b return val)))"
 unfolding AdjustEndian_alt_def
 by PrePost (auto simp: slice_xor)
 
@@ -387,11 +387,11 @@ lemma MemoryInvariant_StoreMemoryCap [MemoryInvariantI]:
                                         return ((needAlign \<and> memType = accessLength) \<or> 
                                                 unat vAddr mod 8 + unat accessLength < 8) \<and>\<^sub>b 
                                         return (a \<notin> Region a' (ucast accessLength + 1)))) \<and>\<^sub>b
-                   (read_state (getMemData a) =\<^sub>b return val))
+                   (read_state (getMemByte a) =\<^sub>b return val))
                  (StoreMemoryCap v)
                  (\<lambda>_. read_state getExceptionSignalled \<or>\<^sub>b
                       read_state isUnpredictable \<or>\<^sub>b
-                      read_state (getMemData a) =\<^sub>b return val)"
+                      read_state (getMemByte a) =\<^sub>b return val)"
 unfolding StoreMemoryCap_alt_def
 by (MemoryInvariant intro: PrePost_DefinedAddressTranslation)
    (auto simp: not_le not_less
@@ -412,11 +412,11 @@ lemma MemoryInvariant_StoreMemory [MemoryInvariantI]:
                                         return ((needAlign \<and> memType = accessLength) \<or> 
                                                 unat vAddr mod 8 + unat accessLength < 8) \<and>\<^sub>b 
                                         return (a \<notin> Region a' (ucast accessLength + 1)))) \<and>\<^sub>b
-                   (read_state (getMemData a) =\<^sub>b return val))
+                   (read_state (getMemByte a) =\<^sub>b return val))
                  (StoreMemory v)
                  (\<lambda>_. read_state getExceptionSignalled \<or>\<^sub>b
                       read_state isUnpredictable \<or>\<^sub>b
-                      read_state (getMemData a) =\<^sub>b return val)"
+                      read_state (getMemByte a) =\<^sub>b return val)"
 unfolding StoreMemory_alt_def 
 by MemoryInvariant auto?
 
@@ -431,17 +431,17 @@ lemma MemoryInvariant_StoreCap [MemoryInvariantI]:
                         (\<lambda>x. case x of None \<Rightarrow> return True
                                      | Some a' \<Rightarrow> return ((cond \<longrightarrow> llbit = Some True) \<longrightarrow>
                                                           (slice 5 a::35 word) \<noteq> slice 5 a')))) \<and>\<^sub>b
-                   (read_state (getMemData a) =\<^sub>b return val))
+                   (read_state (getMemByte a) =\<^sub>b return val))
                  (StoreCap v)
                  (\<lambda>_. read_state getExceptionSignalled \<or>\<^sub>b
                       read_state isUnpredictable \<or>\<^sub>b
-                      read_state (getMemData a) =\<^sub>b return val)"
+                      read_state (getMemByte a) =\<^sub>b return val)"
 proof -
   note addr_trans [MemoryInvariantI] = PrePost_DefinedAddressTranslation
      [where p="\<lambda>x. bind (read_state getLLbit)
                         (\<lambda>llbit. return (((snd (snd v)) \<longrightarrow> llbit = Some True) \<longrightarrow> 
                                           slice 5 a \<noteq> slice 5 x)) \<and>\<^sub>b 
-                   (read_state (getMemData a) =\<^sub>b return val)"]
+                   (read_state (getMemByte a) =\<^sub>b return val)"]
   show ?thesis
     unfolding StoreCap_alt_def 
     by (cases v, strong_cong_simp) MemoryInvariant
@@ -452,403 +452,403 @@ qed
 (* Code generation - skip - Fetch *)
 
 lemma MemoryInvariant_mtc [MemoryInvariantI]:
-  shows "IsInvariant (read_state (getMemData a) =\<^sub>b return val) (mtc v)"
+  shows "IsInvariant (read_state (getMemByte a) =\<^sub>b return val) (mtc v)"
 unfolding mtc_alt_def 
 by MemoryInvariant auto?
 
 lemma MemoryInvariant_dmtc [MemoryInvariantI]:
-  shows "IsInvariant (read_state (getMemData a) =\<^sub>b return val) (dmtc v)"
+  shows "IsInvariant (read_state (getMemByte a) =\<^sub>b return val) (dmtc v)"
 unfolding dmtc_alt_def 
 by MemoryInvariant auto?
 
 lemma MemoryInvariant_mfc [MemoryInvariantI]:
-  shows "IsInvariant (read_state (getMemData a) =\<^sub>b return val) (mfc v)"
+  shows "IsInvariant (read_state (getMemByte a) =\<^sub>b return val) (mfc v)"
 unfolding mfc_alt_def 
 by MemoryInvariant auto?
 
 lemma MemoryInvariant_dmfc [MemoryInvariantI]:
-  shows "IsInvariant (read_state (getMemData a) =\<^sub>b return val) (dmfc v)"
+  shows "IsInvariant (read_state (getMemByte a) =\<^sub>b return val) (dmfc v)"
 unfolding dmfc_alt_def 
 by MemoryInvariant auto?
 
 lemma MemoryInvariant_dfn'ADDI [MemoryInvariantI]:
-  shows "IsInvariant (read_state (getMemData a) =\<^sub>b return val) (dfn'ADDI v)"
+  shows "IsInvariant (read_state (getMemByte a) =\<^sub>b return val) (dfn'ADDI v)"
 unfolding dfn'ADDI_alt_def 
 by MemoryInvariant auto?
 
 lemma MemoryInvariant_dfn'ADDIU [MemoryInvariantI]:
-  shows "IsInvariant (read_state (getMemData a) =\<^sub>b return val) (dfn'ADDIU v)"
+  shows "IsInvariant (read_state (getMemByte a) =\<^sub>b return val) (dfn'ADDIU v)"
 unfolding dfn'ADDIU_alt_def 
 by MemoryInvariant auto?
 
 lemma MemoryInvariant_dfn'DADDI [MemoryInvariantI]:
-  shows "IsInvariant (read_state (getMemData a) =\<^sub>b return val) (dfn'DADDI v)"
+  shows "IsInvariant (read_state (getMemByte a) =\<^sub>b return val) (dfn'DADDI v)"
 unfolding dfn'DADDI_alt_def 
 by MemoryInvariant auto?
 
 lemma MemoryInvariant_dfn'DADDIU [MemoryInvariantI]:
-  shows "IsInvariant (read_state (getMemData a) =\<^sub>b return val) (dfn'DADDIU v)"
+  shows "IsInvariant (read_state (getMemByte a) =\<^sub>b return val) (dfn'DADDIU v)"
 unfolding dfn'DADDIU_alt_def 
 by MemoryInvariant auto?
 
 lemma MemoryInvariant_dfn'SLTI [MemoryInvariantI]:
-  shows "IsInvariant (read_state (getMemData a) =\<^sub>b return val) (dfn'SLTI v)"
+  shows "IsInvariant (read_state (getMemByte a) =\<^sub>b return val) (dfn'SLTI v)"
 unfolding dfn'SLTI_alt_def 
 by MemoryInvariant auto?
 
 lemma MemoryInvariant_dfn'SLTIU [MemoryInvariantI]:
-  shows "IsInvariant (read_state (getMemData a) =\<^sub>b return val) (dfn'SLTIU v)"
+  shows "IsInvariant (read_state (getMemByte a) =\<^sub>b return val) (dfn'SLTIU v)"
 unfolding dfn'SLTIU_alt_def 
 by MemoryInvariant auto?
 
 lemma MemoryInvariant_dfn'ANDI [MemoryInvariantI]:
-  shows "IsInvariant (read_state (getMemData a) =\<^sub>b return val) (dfn'ANDI v)"
+  shows "IsInvariant (read_state (getMemByte a) =\<^sub>b return val) (dfn'ANDI v)"
 unfolding dfn'ANDI_alt_def 
 by MemoryInvariant auto?
 
 lemma MemoryInvariant_dfn'ORI [MemoryInvariantI]:
-  shows "IsInvariant (read_state (getMemData a) =\<^sub>b return val) (dfn'ORI v)"
+  shows "IsInvariant (read_state (getMemByte a) =\<^sub>b return val) (dfn'ORI v)"
 unfolding dfn'ORI_alt_def 
 by MemoryInvariant auto?
 
 lemma MemoryInvariant_dfn'XORI [MemoryInvariantI]:
-  shows "IsInvariant (read_state (getMemData a) =\<^sub>b return val) (dfn'XORI v)"
+  shows "IsInvariant (read_state (getMemByte a) =\<^sub>b return val) (dfn'XORI v)"
 unfolding dfn'XORI_alt_def 
 by MemoryInvariant auto?
 
 lemma MemoryInvariant_dfn'LUI [MemoryInvariantI]:
-  shows "IsInvariant (read_state (getMemData a) =\<^sub>b return val) (dfn'LUI v)"
+  shows "IsInvariant (read_state (getMemByte a) =\<^sub>b return val) (dfn'LUI v)"
 unfolding dfn'LUI_alt_def 
 by MemoryInvariant auto?
 
 lemma MemoryInvariant_dfn'ADD [MemoryInvariantI]:
-  shows "IsInvariant (read_state (getMemData a) =\<^sub>b return val) (dfn'ADD v)"
+  shows "IsInvariant (read_state (getMemByte a) =\<^sub>b return val) (dfn'ADD v)"
 unfolding dfn'ADD_alt_def 
 by MemoryInvariant auto?
 
 lemma MemoryInvariant_dfn'ADDU [MemoryInvariantI]:
-  shows "IsInvariant (read_state (getMemData a) =\<^sub>b return val) (dfn'ADDU v)"
+  shows "IsInvariant (read_state (getMemByte a) =\<^sub>b return val) (dfn'ADDU v)"
 unfolding dfn'ADDU_alt_def 
 by MemoryInvariant auto?
 
 lemma MemoryInvariant_dfn'SUB [MemoryInvariantI]:
-  shows "IsInvariant (read_state (getMemData a) =\<^sub>b return val) (dfn'SUB v)"
+  shows "IsInvariant (read_state (getMemByte a) =\<^sub>b return val) (dfn'SUB v)"
 unfolding dfn'SUB_alt_def 
 by MemoryInvariant auto?
 
 lemma MemoryInvariant_dfn'SUBU [MemoryInvariantI]:
-  shows "IsInvariant (read_state (getMemData a) =\<^sub>b return val) (dfn'SUBU v)"
+  shows "IsInvariant (read_state (getMemByte a) =\<^sub>b return val) (dfn'SUBU v)"
 unfolding dfn'SUBU_alt_def 
 by MemoryInvariant auto?
 
 lemma MemoryInvariant_dfn'DADD [MemoryInvariantI]:
-  shows "IsInvariant (read_state (getMemData a) =\<^sub>b return val) (dfn'DADD v)"
+  shows "IsInvariant (read_state (getMemByte a) =\<^sub>b return val) (dfn'DADD v)"
 unfolding dfn'DADD_alt_def 
 by MemoryInvariant auto?
 
 lemma MemoryInvariant_dfn'DADDU [MemoryInvariantI]:
-  shows "IsInvariant (read_state (getMemData a) =\<^sub>b return val) (dfn'DADDU v)"
+  shows "IsInvariant (read_state (getMemByte a) =\<^sub>b return val) (dfn'DADDU v)"
 unfolding dfn'DADDU_alt_def 
 by MemoryInvariant auto?
 
 lemma MemoryInvariant_dfn'DSUB [MemoryInvariantI]:
-  shows "IsInvariant (read_state (getMemData a) =\<^sub>b return val) (dfn'DSUB v)"
+  shows "IsInvariant (read_state (getMemByte a) =\<^sub>b return val) (dfn'DSUB v)"
 unfolding dfn'DSUB_alt_def 
 by MemoryInvariant auto?
 
 lemma MemoryInvariant_dfn'DSUBU [MemoryInvariantI]:
-  shows "IsInvariant (read_state (getMemData a) =\<^sub>b return val) (dfn'DSUBU v)"
+  shows "IsInvariant (read_state (getMemByte a) =\<^sub>b return val) (dfn'DSUBU v)"
 unfolding dfn'DSUBU_alt_def 
 by MemoryInvariant auto?
 
 lemma MemoryInvariant_dfn'SLT [MemoryInvariantI]:
-  shows "IsInvariant (read_state (getMemData a) =\<^sub>b return val) (dfn'SLT v)"
+  shows "IsInvariant (read_state (getMemByte a) =\<^sub>b return val) (dfn'SLT v)"
 unfolding dfn'SLT_alt_def 
 by MemoryInvariant auto?
 
 lemma MemoryInvariant_dfn'SLTU [MemoryInvariantI]:
-  shows "IsInvariant (read_state (getMemData a) =\<^sub>b return val) (dfn'SLTU v)"
+  shows "IsInvariant (read_state (getMemByte a) =\<^sub>b return val) (dfn'SLTU v)"
 unfolding dfn'SLTU_alt_def 
 by MemoryInvariant auto?
 
 lemma MemoryInvariant_dfn'AND [MemoryInvariantI]:
-  shows "IsInvariant (read_state (getMemData a) =\<^sub>b return val) (dfn'AND v)"
+  shows "IsInvariant (read_state (getMemByte a) =\<^sub>b return val) (dfn'AND v)"
 unfolding dfn'AND_alt_def 
 by MemoryInvariant auto?
 
 lemma MemoryInvariant_dfn'OR [MemoryInvariantI]:
-  shows "IsInvariant (read_state (getMemData a) =\<^sub>b return val) (dfn'OR v)"
+  shows "IsInvariant (read_state (getMemByte a) =\<^sub>b return val) (dfn'OR v)"
 unfolding dfn'OR_alt_def 
 by MemoryInvariant auto?
 
 lemma MemoryInvariant_dfn'XOR [MemoryInvariantI]:
-  shows "IsInvariant (read_state (getMemData a) =\<^sub>b return val) (dfn'XOR v)"
+  shows "IsInvariant (read_state (getMemByte a) =\<^sub>b return val) (dfn'XOR v)"
 unfolding dfn'XOR_alt_def 
 by MemoryInvariant auto?
 
 lemma MemoryInvariant_dfn'NOR [MemoryInvariantI]:
-  shows "IsInvariant (read_state (getMemData a) =\<^sub>b return val) (dfn'NOR v)"
+  shows "IsInvariant (read_state (getMemByte a) =\<^sub>b return val) (dfn'NOR v)"
 unfolding dfn'NOR_alt_def 
 by MemoryInvariant auto?
 
 lemma MemoryInvariant_dfn'MOVN [MemoryInvariantI]:
-  shows "IsInvariant (read_state (getMemData a) =\<^sub>b return val) (dfn'MOVN v)"
+  shows "IsInvariant (read_state (getMemByte a) =\<^sub>b return val) (dfn'MOVN v)"
 unfolding dfn'MOVN_alt_def 
 by MemoryInvariant auto?
 
 lemma MemoryInvariant_dfn'MOVZ [MemoryInvariantI]:
-  shows "IsInvariant (read_state (getMemData a) =\<^sub>b return val) (dfn'MOVZ v)"
+  shows "IsInvariant (read_state (getMemByte a) =\<^sub>b return val) (dfn'MOVZ v)"
 unfolding dfn'MOVZ_alt_def 
 by MemoryInvariant auto?
 
 lemma MemoryInvariant_dfn'MADD [MemoryInvariantI]:
-  shows "IsInvariant (read_state (getMemData a) =\<^sub>b return val) (dfn'MADD v)"
+  shows "IsInvariant (read_state (getMemByte a) =\<^sub>b return val) (dfn'MADD v)"
 unfolding dfn'MADD_alt_def 
 by MemoryInvariant auto?
 
 lemma MemoryInvariant_dfn'MADDU [MemoryInvariantI]:
-  shows "IsInvariant (read_state (getMemData a) =\<^sub>b return val) (dfn'MADDU v)"
+  shows "IsInvariant (read_state (getMemByte a) =\<^sub>b return val) (dfn'MADDU v)"
 unfolding dfn'MADDU_alt_def 
 by MemoryInvariant auto?
 
 lemma MemoryInvariant_dfn'MSUB [MemoryInvariantI]:
-  shows "IsInvariant (read_state (getMemData a) =\<^sub>b return val) (dfn'MSUB v)"
+  shows "IsInvariant (read_state (getMemByte a) =\<^sub>b return val) (dfn'MSUB v)"
 unfolding dfn'MSUB_alt_def 
 by MemoryInvariant auto?
 
 lemma MemoryInvariant_dfn'MSUBU [MemoryInvariantI]:
-  shows "IsInvariant (read_state (getMemData a) =\<^sub>b return val) (dfn'MSUBU v)"
+  shows "IsInvariant (read_state (getMemByte a) =\<^sub>b return val) (dfn'MSUBU v)"
 unfolding dfn'MSUBU_alt_def 
 by MemoryInvariant auto?
 
 lemma MemoryInvariant_dfn'MUL [MemoryInvariantI]:
-  shows "IsInvariant (read_state (getMemData a) =\<^sub>b return val) (dfn'MUL v)"
+  shows "IsInvariant (read_state (getMemByte a) =\<^sub>b return val) (dfn'MUL v)"
 unfolding dfn'MUL_alt_def 
 by MemoryInvariant auto?
 
 lemma MemoryInvariant_dfn'MULT [MemoryInvariantI]:
-  shows "IsInvariant (read_state (getMemData a) =\<^sub>b return val) (dfn'MULT v)"
+  shows "IsInvariant (read_state (getMemByte a) =\<^sub>b return val) (dfn'MULT v)"
 unfolding dfn'MULT_alt_def 
 by MemoryInvariant auto?
 
 lemma MemoryInvariant_dfn'MULTU [MemoryInvariantI]:
-  shows "IsInvariant (read_state (getMemData a) =\<^sub>b return val) (dfn'MULTU v)"
+  shows "IsInvariant (read_state (getMemByte a) =\<^sub>b return val) (dfn'MULTU v)"
 unfolding dfn'MULTU_alt_def 
 by MemoryInvariant auto?
 
 lemma MemoryInvariant_dfn'DMULT [MemoryInvariantI]:
-  shows "IsInvariant (read_state (getMemData a) =\<^sub>b return val) (dfn'DMULT v)"
+  shows "IsInvariant (read_state (getMemByte a) =\<^sub>b return val) (dfn'DMULT v)"
 unfolding dfn'DMULT_alt_def 
 by MemoryInvariant auto?
 
 lemma MemoryInvariant_dfn'DMULTU [MemoryInvariantI]:
-  shows "IsInvariant (read_state (getMemData a) =\<^sub>b return val) (dfn'DMULTU v)"
+  shows "IsInvariant (read_state (getMemByte a) =\<^sub>b return val) (dfn'DMULTU v)"
 unfolding dfn'DMULTU_alt_def 
 by MemoryInvariant auto?
 
 lemma MemoryInvariant_dfn'DIV [MemoryInvariantI]:
-  shows "IsInvariant (read_state (getMemData a) =\<^sub>b return val) (dfn'DIV v)"
+  shows "IsInvariant (read_state (getMemByte a) =\<^sub>b return val) (dfn'DIV v)"
 unfolding dfn'DIV_alt_def 
 by MemoryInvariant auto?
 
 lemma MemoryInvariant_dfn'DIVU [MemoryInvariantI]:
-  shows "IsInvariant (read_state (getMemData a) =\<^sub>b return val) (dfn'DIVU v)"
+  shows "IsInvariant (read_state (getMemByte a) =\<^sub>b return val) (dfn'DIVU v)"
 unfolding dfn'DIVU_alt_def 
 by MemoryInvariant auto?
 
 lemma MemoryInvariant_dfn'DDIV [MemoryInvariantI]:
-  shows "IsInvariant (read_state (getMemData a) =\<^sub>b return val) (dfn'DDIV v)"
+  shows "IsInvariant (read_state (getMemByte a) =\<^sub>b return val) (dfn'DDIV v)"
 unfolding dfn'DDIV_alt_def 
 by MemoryInvariant auto?
 
 lemma MemoryInvariant_dfn'DDIVU [MemoryInvariantI]:
-  shows "IsInvariant (read_state (getMemData a) =\<^sub>b return val) (dfn'DDIVU v)"
+  shows "IsInvariant (read_state (getMemByte a) =\<^sub>b return val) (dfn'DDIVU v)"
 unfolding dfn'DDIVU_alt_def 
 by MemoryInvariant auto?
 
 lemma MemoryInvariant_dfn'MFHI [MemoryInvariantI]:
-  shows "IsInvariant (read_state (getMemData a) =\<^sub>b return val) (dfn'MFHI v)"
+  shows "IsInvariant (read_state (getMemByte a) =\<^sub>b return val) (dfn'MFHI v)"
 unfolding dfn'MFHI_alt_def 
 by MemoryInvariant auto?
 
 lemma MemoryInvariant_dfn'MFLO [MemoryInvariantI]:
-  shows "IsInvariant (read_state (getMemData a) =\<^sub>b return val) (dfn'MFLO v)"
+  shows "IsInvariant (read_state (getMemByte a) =\<^sub>b return val) (dfn'MFLO v)"
 unfolding dfn'MFLO_alt_def 
 by MemoryInvariant auto?
 
 lemma MemoryInvariant_dfn'MTHI [MemoryInvariantI]:
-  shows "IsInvariant (read_state (getMemData a) =\<^sub>b return val) (dfn'MTHI v)"
+  shows "IsInvariant (read_state (getMemByte a) =\<^sub>b return val) (dfn'MTHI v)"
 unfolding dfn'MTHI_alt_def 
 by MemoryInvariant auto?
 
 lemma MemoryInvariant_dfn'MTLO [MemoryInvariantI]:
-  shows "IsInvariant (read_state (getMemData a) =\<^sub>b return val) (dfn'MTLO v)"
+  shows "IsInvariant (read_state (getMemByte a) =\<^sub>b return val) (dfn'MTLO v)"
 unfolding dfn'MTLO_alt_def 
 by MemoryInvariant auto?
 
 lemma MemoryInvariant_dfn'SLL [MemoryInvariantI]:
-  shows "IsInvariant (read_state (getMemData a) =\<^sub>b return val) (dfn'SLL v)"
+  shows "IsInvariant (read_state (getMemByte a) =\<^sub>b return val) (dfn'SLL v)"
 unfolding dfn'SLL_alt_def 
 by MemoryInvariant auto?
 
 lemma MemoryInvariant_dfn'SRL [MemoryInvariantI]:
-  shows "IsInvariant (read_state (getMemData a) =\<^sub>b return val) (dfn'SRL v)"
+  shows "IsInvariant (read_state (getMemByte a) =\<^sub>b return val) (dfn'SRL v)"
 unfolding dfn'SRL_alt_def 
 by MemoryInvariant auto?
 
 lemma MemoryInvariant_dfn'SRA [MemoryInvariantI]:
-  shows "IsInvariant (read_state (getMemData a) =\<^sub>b return val) (dfn'SRA v)"
+  shows "IsInvariant (read_state (getMemByte a) =\<^sub>b return val) (dfn'SRA v)"
 unfolding dfn'SRA_alt_def 
 by MemoryInvariant auto?
 
 lemma MemoryInvariant_dfn'SLLV [MemoryInvariantI]:
-  shows "IsInvariant (read_state (getMemData a) =\<^sub>b return val) (dfn'SLLV v)"
+  shows "IsInvariant (read_state (getMemByte a) =\<^sub>b return val) (dfn'SLLV v)"
 unfolding dfn'SLLV_alt_def 
 by MemoryInvariant auto?
 
 lemma MemoryInvariant_dfn'SRLV [MemoryInvariantI]:
-  shows "IsInvariant (read_state (getMemData a) =\<^sub>b return val) (dfn'SRLV v)"
+  shows "IsInvariant (read_state (getMemByte a) =\<^sub>b return val) (dfn'SRLV v)"
 unfolding dfn'SRLV_alt_def 
 by MemoryInvariant auto?
 
 lemma MemoryInvariant_dfn'SRAV [MemoryInvariantI]:
-  shows "IsInvariant (read_state (getMemData a) =\<^sub>b return val) (dfn'SRAV v)"
+  shows "IsInvariant (read_state (getMemByte a) =\<^sub>b return val) (dfn'SRAV v)"
 unfolding dfn'SRAV_alt_def 
 by MemoryInvariant auto?
 
 lemma MemoryInvariant_dfn'DSLL [MemoryInvariantI]:
-  shows "IsInvariant (read_state (getMemData a) =\<^sub>b return val) (dfn'DSLL v)"
+  shows "IsInvariant (read_state (getMemByte a) =\<^sub>b return val) (dfn'DSLL v)"
 unfolding dfn'DSLL_alt_def 
 by MemoryInvariant auto?
 
 lemma MemoryInvariant_dfn'DSRL [MemoryInvariantI]:
-  shows "IsInvariant (read_state (getMemData a) =\<^sub>b return val) (dfn'DSRL v)"
+  shows "IsInvariant (read_state (getMemByte a) =\<^sub>b return val) (dfn'DSRL v)"
 unfolding dfn'DSRL_alt_def 
 by MemoryInvariant auto?
 
 lemma MemoryInvariant_dfn'DSRA [MemoryInvariantI]:
-  shows "IsInvariant (read_state (getMemData a) =\<^sub>b return val) (dfn'DSRA v)"
+  shows "IsInvariant (read_state (getMemByte a) =\<^sub>b return val) (dfn'DSRA v)"
 unfolding dfn'DSRA_alt_def 
 by MemoryInvariant auto?
 
 lemma MemoryInvariant_dfn'DSLLV [MemoryInvariantI]:
-  shows "IsInvariant (read_state (getMemData a) =\<^sub>b return val) (dfn'DSLLV v)"
+  shows "IsInvariant (read_state (getMemByte a) =\<^sub>b return val) (dfn'DSLLV v)"
 unfolding dfn'DSLLV_alt_def 
 by MemoryInvariant auto?
 
 lemma MemoryInvariant_dfn'DSRLV [MemoryInvariantI]:
-  shows "IsInvariant (read_state (getMemData a) =\<^sub>b return val) (dfn'DSRLV v)"
+  shows "IsInvariant (read_state (getMemByte a) =\<^sub>b return val) (dfn'DSRLV v)"
 unfolding dfn'DSRLV_alt_def 
 by MemoryInvariant auto?
 
 lemma MemoryInvariant_dfn'DSRAV [MemoryInvariantI]:
-  shows "IsInvariant (read_state (getMemData a) =\<^sub>b return val) (dfn'DSRAV v)"
+  shows "IsInvariant (read_state (getMemByte a) =\<^sub>b return val) (dfn'DSRAV v)"
 unfolding dfn'DSRAV_alt_def 
 by MemoryInvariant auto?
 
 lemma MemoryInvariant_dfn'DSLL32 [MemoryInvariantI]:
-  shows "IsInvariant (read_state (getMemData a) =\<^sub>b return val) (dfn'DSLL32 v)"
+  shows "IsInvariant (read_state (getMemByte a) =\<^sub>b return val) (dfn'DSLL32 v)"
 unfolding dfn'DSLL32_alt_def 
 by MemoryInvariant auto?
 
 lemma MemoryInvariant_dfn'DSRL32 [MemoryInvariantI]:
-  shows "IsInvariant (read_state (getMemData a) =\<^sub>b return val) (dfn'DSRL32 v)"
+  shows "IsInvariant (read_state (getMemByte a) =\<^sub>b return val) (dfn'DSRL32 v)"
 unfolding dfn'DSRL32_alt_def 
 by MemoryInvariant auto?
 
 lemma MemoryInvariant_dfn'DSRA32 [MemoryInvariantI]:
-  shows "IsInvariant (read_state (getMemData a) =\<^sub>b return val) (dfn'DSRA32 v)"
+  shows "IsInvariant (read_state (getMemByte a) =\<^sub>b return val) (dfn'DSRA32 v)"
 unfolding dfn'DSRA32_alt_def 
 by MemoryInvariant auto?
 
 lemma MemoryInvariant_dfn'TGE [MemoryInvariantI]:
-  shows "IsInvariant (read_state (getMemData a) =\<^sub>b return val) (dfn'TGE v)"
+  shows "IsInvariant (read_state (getMemByte a) =\<^sub>b return val) (dfn'TGE v)"
 unfolding dfn'TGE_alt_def 
 by MemoryInvariant auto?
 
 lemma MemoryInvariant_dfn'TGEU [MemoryInvariantI]:
-  shows "IsInvariant (read_state (getMemData a) =\<^sub>b return val) (dfn'TGEU v)"
+  shows "IsInvariant (read_state (getMemByte a) =\<^sub>b return val) (dfn'TGEU v)"
 unfolding dfn'TGEU_alt_def 
 by MemoryInvariant auto?
 
 lemma MemoryInvariant_dfn'TLT [MemoryInvariantI]:
-  shows "IsInvariant (read_state (getMemData a) =\<^sub>b return val) (dfn'TLT v)"
+  shows "IsInvariant (read_state (getMemByte a) =\<^sub>b return val) (dfn'TLT v)"
 unfolding dfn'TLT_alt_def 
 by MemoryInvariant auto?
 
 lemma MemoryInvariant_dfn'TLTU [MemoryInvariantI]:
-  shows "IsInvariant (read_state (getMemData a) =\<^sub>b return val) (dfn'TLTU v)"
+  shows "IsInvariant (read_state (getMemByte a) =\<^sub>b return val) (dfn'TLTU v)"
 unfolding dfn'TLTU_alt_def 
 by MemoryInvariant auto?
 
 lemma MemoryInvariant_dfn'TEQ [MemoryInvariantI]:
-  shows "IsInvariant (read_state (getMemData a) =\<^sub>b return val) (dfn'TEQ v)"
+  shows "IsInvariant (read_state (getMemByte a) =\<^sub>b return val) (dfn'TEQ v)"
 unfolding dfn'TEQ_alt_def 
 by MemoryInvariant auto?
 
 lemma MemoryInvariant_dfn'TNE [MemoryInvariantI]:
-  shows "IsInvariant (read_state (getMemData a) =\<^sub>b return val) (dfn'TNE v)"
+  shows "IsInvariant (read_state (getMemByte a) =\<^sub>b return val) (dfn'TNE v)"
 unfolding dfn'TNE_alt_def 
 by MemoryInvariant auto?
 
 lemma MemoryInvariant_dfn'TGEI [MemoryInvariantI]:
-  shows "IsInvariant (read_state (getMemData a) =\<^sub>b return val) (dfn'TGEI v)"
+  shows "IsInvariant (read_state (getMemByte a) =\<^sub>b return val) (dfn'TGEI v)"
 unfolding dfn'TGEI_alt_def 
 by MemoryInvariant auto?
 
 lemma MemoryInvariant_dfn'TGEIU [MemoryInvariantI]:
-  shows "IsInvariant (read_state (getMemData a) =\<^sub>b return val) (dfn'TGEIU v)"
+  shows "IsInvariant (read_state (getMemByte a) =\<^sub>b return val) (dfn'TGEIU v)"
 unfolding dfn'TGEIU_alt_def 
 by MemoryInvariant auto?
 
 lemma MemoryInvariant_dfn'TLTI [MemoryInvariantI]:
-  shows "IsInvariant (read_state (getMemData a) =\<^sub>b return val) (dfn'TLTI v)"
+  shows "IsInvariant (read_state (getMemByte a) =\<^sub>b return val) (dfn'TLTI v)"
 unfolding dfn'TLTI_alt_def 
 by MemoryInvariant auto?
 
 lemma MemoryInvariant_dfn'TLTIU [MemoryInvariantI]:
-  shows "IsInvariant (read_state (getMemData a) =\<^sub>b return val) (dfn'TLTIU v)"
+  shows "IsInvariant (read_state (getMemByte a) =\<^sub>b return val) (dfn'TLTIU v)"
 unfolding dfn'TLTIU_alt_def 
 by MemoryInvariant auto?
 
 lemma MemoryInvariant_dfn'TEQI [MemoryInvariantI]:
-  shows "IsInvariant (read_state (getMemData a) =\<^sub>b return val) (dfn'TEQI v)"
+  shows "IsInvariant (read_state (getMemByte a) =\<^sub>b return val) (dfn'TEQI v)"
 unfolding dfn'TEQI_alt_def 
 by MemoryInvariant auto?
 
 lemma MemoryInvariant_dfn'TNEI [MemoryInvariantI]:
-  shows "IsInvariant (read_state (getMemData a) =\<^sub>b return val) (dfn'TNEI v)"
+  shows "IsInvariant (read_state (getMemByte a) =\<^sub>b return val) (dfn'TNEI v)"
 unfolding dfn'TNEI_alt_def 
 by MemoryInvariant auto?
 
 lemma MemoryInvariant_loadByte [MemoryInvariantI]:
-  shows "IsInvariant (read_state (getMemData a) =\<^sub>b return val) (loadByte v)"
+  shows "IsInvariant (read_state (getMemByte a) =\<^sub>b return val) (loadByte v)"
 unfolding loadByte_alt_def 
 by MemoryInvariant auto?
 
 lemma MemoryInvariant_loadHalf [MemoryInvariantI]:
-  shows "IsInvariant (read_state (getMemData a) =\<^sub>b return val) (loadHalf v)"
+  shows "IsInvariant (read_state (getMemByte a) =\<^sub>b return val) (loadHalf v)"
 unfolding loadHalf_alt_def 
 by MemoryInvariant auto?
 
 lemma MemoryInvariant_loadWord [MemoryInvariantI]:
-  shows "IsInvariant (read_state (getMemData a) =\<^sub>b return val) (loadWord v)"
+  shows "IsInvariant (read_state (getMemByte a) =\<^sub>b return val) (loadWord v)"
 unfolding loadWord_alt_def 
 by MemoryInvariant auto?
 
 lemma MemoryInvariant_loadDoubleword [MemoryInvariantI]:
-  shows "IsInvariant (read_state (getMemData a) =\<^sub>b return val) (loadDoubleword v)"
+  shows "IsInvariant (read_state (getMemByte a) =\<^sub>b return val) (loadDoubleword v)"
 unfolding loadDoubleword_alt_def 
 by MemoryInvariant auto?
 
 lemma MemoryInvariant_dfn'LB [MemoryInvariantI]:
-  shows "PrePost ((read_state (getMemData a) =\<^sub>b return val) \<and>\<^sub>b
+  shows "PrePost ((read_state (getMemByte a) =\<^sub>b return val) \<and>\<^sub>b
                   bind (LBActions v)
                        (\<lambda>p. return (a \<notin> \<Union> (WrittenAddresses ` p))))
                  (dfn'LB v)
                  (\<lambda>_. read_state getExceptionSignalled \<or>\<^sub>b
                       read_state isUnpredictable \<or>\<^sub>b
-                      read_state (getMemData a) =\<^sub>b return val)"
+                      read_state (getMemByte a) =\<^sub>b return val)"
 unfolding dfn'LB_alt_def LBActions_def 
 unfolding LegacyStoreActions_def LegacyStorePhysicalAddress_def LegacyStoreVirtualAddress_def
 unfolding BYTE_def HALFWORD_def WORD_def DOUBLEWORD_def
@@ -856,13 +856,13 @@ unfolding CheckBranch_alt_def getVirtualAddress_alt_def
 by MemoryInvariant auto?
 
 lemma MemoryInvariant_dfn'LBU [MemoryInvariantI]:
-  shows "PrePost ((read_state (getMemData a) =\<^sub>b return val) \<and>\<^sub>b
+  shows "PrePost ((read_state (getMemByte a) =\<^sub>b return val) \<and>\<^sub>b
                   bind (LBUActions v)
                        (\<lambda>p. return (a \<notin> \<Union> (WrittenAddresses ` p))))
                  (dfn'LBU v)
                  (\<lambda>_. read_state getExceptionSignalled \<or>\<^sub>b
                       read_state isUnpredictable \<or>\<^sub>b
-                      read_state (getMemData a) =\<^sub>b return val)"
+                      read_state (getMemByte a) =\<^sub>b return val)"
 unfolding dfn'LBU_alt_def LBUActions_def 
 unfolding LegacyStoreActions_def LegacyStorePhysicalAddress_def LegacyStoreVirtualAddress_def
 unfolding BYTE_def HALFWORD_def WORD_def DOUBLEWORD_def
@@ -870,13 +870,13 @@ unfolding CheckBranch_alt_def getVirtualAddress_alt_def
 by MemoryInvariant auto?
 
 lemma MemoryInvariant_dfn'LH [MemoryInvariantI]:
-  shows "PrePost ((read_state (getMemData a) =\<^sub>b return val) \<and>\<^sub>b
+  shows "PrePost ((read_state (getMemByte a) =\<^sub>b return val) \<and>\<^sub>b
                   bind (LHActions v)
                        (\<lambda>p. return (a \<notin> \<Union> (WrittenAddresses ` p))))
                  (dfn'LH v)
                  (\<lambda>_. read_state getExceptionSignalled \<or>\<^sub>b
                       read_state isUnpredictable \<or>\<^sub>b
-                      read_state (getMemData a) =\<^sub>b return val)"
+                      read_state (getMemByte a) =\<^sub>b return val)"
 unfolding dfn'LH_alt_def LHActions_def 
 unfolding LegacyStoreActions_def LegacyStorePhysicalAddress_def LegacyStoreVirtualAddress_def
 unfolding BYTE_def HALFWORD_def WORD_def DOUBLEWORD_def
@@ -884,13 +884,13 @@ unfolding CheckBranch_alt_def getVirtualAddress_alt_def
 by MemoryInvariant auto?
 
 lemma MemoryInvariant_dfn'LHU [MemoryInvariantI]:
-  shows "PrePost ((read_state (getMemData a) =\<^sub>b return val) \<and>\<^sub>b
+  shows "PrePost ((read_state (getMemByte a) =\<^sub>b return val) \<and>\<^sub>b
                   bind (LHUActions v)
                        (\<lambda>p. return (a \<notin> \<Union> (WrittenAddresses ` p))))
                  (dfn'LHU v)
                  (\<lambda>_. read_state getExceptionSignalled \<or>\<^sub>b
                       read_state isUnpredictable \<or>\<^sub>b
-                      read_state (getMemData a) =\<^sub>b return val)"
+                      read_state (getMemByte a) =\<^sub>b return val)"
 unfolding dfn'LHU_alt_def LHUActions_def 
 unfolding LegacyStoreActions_def LegacyStorePhysicalAddress_def LegacyStoreVirtualAddress_def
 unfolding BYTE_def HALFWORD_def WORD_def DOUBLEWORD_def
@@ -898,13 +898,13 @@ unfolding CheckBranch_alt_def getVirtualAddress_alt_def
 by MemoryInvariant auto?
 
 lemma MemoryInvariant_dfn'LW [MemoryInvariantI]:
-  shows "PrePost ((read_state (getMemData a) =\<^sub>b return val) \<and>\<^sub>b
+  shows "PrePost ((read_state (getMemByte a) =\<^sub>b return val) \<and>\<^sub>b
                   bind (LWActions v)
                        (\<lambda>p. return (a \<notin> \<Union> (WrittenAddresses ` p))))
                  (dfn'LW v)
                  (\<lambda>_. read_state getExceptionSignalled \<or>\<^sub>b
                       read_state isUnpredictable \<or>\<^sub>b
-                      read_state (getMemData a) =\<^sub>b return val)"
+                      read_state (getMemByte a) =\<^sub>b return val)"
 unfolding dfn'LW_alt_def LWActions_def 
 unfolding LegacyStoreActions_def LegacyStorePhysicalAddress_def LegacyStoreVirtualAddress_def
 unfolding BYTE_def HALFWORD_def WORD_def DOUBLEWORD_def
@@ -912,13 +912,13 @@ unfolding CheckBranch_alt_def getVirtualAddress_alt_def
 by MemoryInvariant auto?
 
 lemma MemoryInvariant_dfn'LWU [MemoryInvariantI]:
-  shows "PrePost ((read_state (getMemData a) =\<^sub>b return val) \<and>\<^sub>b
+  shows "PrePost ((read_state (getMemByte a) =\<^sub>b return val) \<and>\<^sub>b
                   bind (LWUActions v)
                        (\<lambda>p. return (a \<notin> \<Union> (WrittenAddresses ` p))))
                  (dfn'LWU v)
                  (\<lambda>_. read_state getExceptionSignalled \<or>\<^sub>b
                       read_state isUnpredictable \<or>\<^sub>b
-                      read_state (getMemData a) =\<^sub>b return val)"
+                      read_state (getMemByte a) =\<^sub>b return val)"
 unfolding dfn'LWU_alt_def LWUActions_def 
 unfolding LegacyStoreActions_def LegacyStorePhysicalAddress_def LegacyStoreVirtualAddress_def
 unfolding BYTE_def HALFWORD_def WORD_def DOUBLEWORD_def
@@ -926,13 +926,13 @@ unfolding CheckBranch_alt_def getVirtualAddress_alt_def
 by MemoryInvariant auto?
 
 lemma MemoryInvariant_dfn'LL [MemoryInvariantI]:
-  shows "PrePost ((read_state (getMemData a) =\<^sub>b return val) \<and>\<^sub>b
+  shows "PrePost ((read_state (getMemByte a) =\<^sub>b return val) \<and>\<^sub>b
                   bind (LLActions v)
                        (\<lambda>p. return (a \<notin> \<Union> (WrittenAddresses ` p))))
                  (dfn'LL v)
                  (\<lambda>_. read_state getExceptionSignalled \<or>\<^sub>b
                       read_state isUnpredictable \<or>\<^sub>b
-                      read_state (getMemData a) =\<^sub>b return val)"
+                      read_state (getMemByte a) =\<^sub>b return val)"
 unfolding dfn'LL_alt_def LLActions_def 
 unfolding LegacyStoreActions_def LegacyStorePhysicalAddress_def LegacyStoreVirtualAddress_def
 unfolding BYTE_def HALFWORD_def WORD_def DOUBLEWORD_def
@@ -940,13 +940,13 @@ unfolding CheckBranch_alt_def getVirtualAddress_alt_def
 by MemoryInvariant auto?
 
 lemma MemoryInvariant_dfn'LD [MemoryInvariantI]:
-  shows "PrePost ((read_state (getMemData a) =\<^sub>b return val) \<and>\<^sub>b
+  shows "PrePost ((read_state (getMemByte a) =\<^sub>b return val) \<and>\<^sub>b
                   bind (LDActions v)
                        (\<lambda>p. return (a \<notin> \<Union> (WrittenAddresses ` p))))
                  (dfn'LD v)
                  (\<lambda>_. read_state getExceptionSignalled \<or>\<^sub>b
                       read_state isUnpredictable \<or>\<^sub>b
-                      read_state (getMemData a) =\<^sub>b return val)"
+                      read_state (getMemByte a) =\<^sub>b return val)"
 unfolding dfn'LD_alt_def LDActions_def 
 unfolding LegacyStoreActions_def LegacyStorePhysicalAddress_def LegacyStoreVirtualAddress_def
 unfolding BYTE_def HALFWORD_def WORD_def DOUBLEWORD_def
@@ -954,13 +954,13 @@ unfolding CheckBranch_alt_def getVirtualAddress_alt_def
 by MemoryInvariant auto?
 
 lemma MemoryInvariant_dfn'LLD [MemoryInvariantI]:
-  shows "PrePost ((read_state (getMemData a) =\<^sub>b return val) \<and>\<^sub>b
+  shows "PrePost ((read_state (getMemByte a) =\<^sub>b return val) \<and>\<^sub>b
                   bind (LLDActions v)
                        (\<lambda>p. return (a \<notin> \<Union> (WrittenAddresses ` p))))
                  (dfn'LLD v)
                  (\<lambda>_. read_state getExceptionSignalled \<or>\<^sub>b
                       read_state isUnpredictable \<or>\<^sub>b
-                      read_state (getMemData a) =\<^sub>b return val)"
+                      read_state (getMemByte a) =\<^sub>b return val)"
 unfolding dfn'LLD_alt_def LLDActions_def 
 unfolding LegacyStoreActions_def LegacyStorePhysicalAddress_def LegacyStoreVirtualAddress_def
 unfolding BYTE_def HALFWORD_def WORD_def DOUBLEWORD_def
@@ -968,13 +968,13 @@ unfolding CheckBranch_alt_def getVirtualAddress_alt_def
 by MemoryInvariant auto?
 
 lemma MemoryInvariant_dfn'LWL [MemoryInvariantI]:
-  shows "PrePost ((read_state (getMemData a) =\<^sub>b return val) \<and>\<^sub>b
+  shows "PrePost ((read_state (getMemByte a) =\<^sub>b return val) \<and>\<^sub>b
                   bind (LWLActions v)
                        (\<lambda>p. return (a \<notin> \<Union> (WrittenAddresses ` p))))
                  (dfn'LWL v)
                  (\<lambda>_. read_state getExceptionSignalled \<or>\<^sub>b
                       read_state isUnpredictable \<or>\<^sub>b
-                      read_state (getMemData a) =\<^sub>b return val)"
+                      read_state (getMemByte a) =\<^sub>b return val)"
 unfolding dfn'LWL_alt_def LWLActions_def 
 unfolding LegacyStoreActions_def LegacyStorePhysicalAddress_def LegacyStoreVirtualAddress_def
 unfolding BYTE_def HALFWORD_def WORD_def DOUBLEWORD_def
@@ -982,13 +982,13 @@ unfolding CheckBranch_alt_def getVirtualAddress_alt_def
 by MemoryInvariant auto?
 
 lemma MemoryInvariant_dfn'LWR [MemoryInvariantI]:
-  shows "PrePost ((read_state (getMemData a) =\<^sub>b return val) \<and>\<^sub>b
+  shows "PrePost ((read_state (getMemByte a) =\<^sub>b return val) \<and>\<^sub>b
                   bind (LWRActions v)
                        (\<lambda>p. return (a \<notin> \<Union> (WrittenAddresses ` p))))
                  (dfn'LWR v)
                  (\<lambda>_. read_state getExceptionSignalled \<or>\<^sub>b
                       read_state isUnpredictable \<or>\<^sub>b
-                      read_state (getMemData a) =\<^sub>b return val)"
+                      read_state (getMemByte a) =\<^sub>b return val)"
 unfolding dfn'LWR_alt_def LWRActions_def 
 unfolding LegacyStoreActions_def LegacyStorePhysicalAddress_def LegacyStoreVirtualAddress_def
 unfolding BYTE_def HALFWORD_def WORD_def DOUBLEWORD_def
@@ -996,13 +996,13 @@ unfolding CheckBranch_alt_def getVirtualAddress_alt_def
 by MemoryInvariant auto?
 
 lemma MemoryInvariant_dfn'LDL [MemoryInvariantI]:
-  shows "PrePost ((read_state (getMemData a) =\<^sub>b return val) \<and>\<^sub>b
+  shows "PrePost ((read_state (getMemByte a) =\<^sub>b return val) \<and>\<^sub>b
                   bind (LDLActions v)
                        (\<lambda>p. return (a \<notin> \<Union> (WrittenAddresses ` p))))
                  (dfn'LDL v)
                  (\<lambda>_. read_state getExceptionSignalled \<or>\<^sub>b
                       read_state isUnpredictable \<or>\<^sub>b
-                      read_state (getMemData a) =\<^sub>b return val)"
+                      read_state (getMemByte a) =\<^sub>b return val)"
 unfolding dfn'LDL_alt_def LDLActions_def 
 unfolding LegacyStoreActions_def LegacyStorePhysicalAddress_def LegacyStoreVirtualAddress_def
 unfolding BYTE_def HALFWORD_def WORD_def DOUBLEWORD_def
@@ -1010,13 +1010,13 @@ unfolding CheckBranch_alt_def getVirtualAddress_alt_def
 by MemoryInvariant auto?
 
 lemma MemoryInvariant_dfn'LDR [MemoryInvariantI]:
-  shows "PrePost ((read_state (getMemData a) =\<^sub>b return val) \<and>\<^sub>b
+  shows "PrePost ((read_state (getMemByte a) =\<^sub>b return val) \<and>\<^sub>b
                   bind (LDRActions v)
                        (\<lambda>p. return (a \<notin> \<Union> (WrittenAddresses ` p))))
                  (dfn'LDR v)
                  (\<lambda>_. read_state getExceptionSignalled \<or>\<^sub>b
                       read_state isUnpredictable \<or>\<^sub>b
-                      read_state (getMemData a) =\<^sub>b return val)"
+                      read_state (getMemByte a) =\<^sub>b return val)"
 unfolding dfn'LDR_alt_def LDRActions_def 
 unfolding LegacyStoreActions_def LegacyStorePhysicalAddress_def LegacyStoreVirtualAddress_def
 unfolding BYTE_def HALFWORD_def WORD_def DOUBLEWORD_def
@@ -1024,13 +1024,13 @@ unfolding CheckBranch_alt_def getVirtualAddress_alt_def
 by MemoryInvariant auto?
 
 lemma MemoryInvariant_dfn'SB [MemoryInvariantI]:
-  shows "PrePost ((read_state (getMemData a) =\<^sub>b return val) \<and>\<^sub>b
+  shows "PrePost ((read_state (getMemByte a) =\<^sub>b return val) \<and>\<^sub>b
                   bind (SBActions v)
                        (\<lambda>p. return (a \<notin> \<Union> (WrittenAddresses ` p))))
                  (dfn'SB v)
                  (\<lambda>_. read_state getExceptionSignalled \<or>\<^sub>b
                       read_state isUnpredictable \<or>\<^sub>b
-                      read_state (getMemData a) =\<^sub>b return val)"
+                      read_state (getMemByte a) =\<^sub>b return val)"
 unfolding dfn'SB_alt_def SBActions_def 
 unfolding LegacyStoreActions_def LegacyStorePhysicalAddress_def LegacyStoreVirtualAddress_def
 unfolding BYTE_def HALFWORD_def WORD_def DOUBLEWORD_def
@@ -1038,13 +1038,13 @@ unfolding CheckBranch_alt_def getVirtualAddress_alt_def
 by MemoryInvariant auto?
 
 lemma MemoryInvariant_dfn'SH [MemoryInvariantI]:
-  shows "PrePost ((read_state (getMemData a) =\<^sub>b return val) \<and>\<^sub>b
+  shows "PrePost ((read_state (getMemByte a) =\<^sub>b return val) \<and>\<^sub>b
                   bind (SHActions v)
                        (\<lambda>p. return (a \<notin> \<Union> (WrittenAddresses ` p))))
                  (dfn'SH v)
                  (\<lambda>_. read_state getExceptionSignalled \<or>\<^sub>b
                       read_state isUnpredictable \<or>\<^sub>b
-                      read_state (getMemData a) =\<^sub>b return val)"
+                      read_state (getMemByte a) =\<^sub>b return val)"
 unfolding dfn'SH_alt_def SHActions_def 
 unfolding LegacyStoreActions_def LegacyStorePhysicalAddress_def LegacyStoreVirtualAddress_def
 unfolding BYTE_def HALFWORD_def WORD_def DOUBLEWORD_def
@@ -1061,11 +1061,11 @@ lemma MemoryInvariant_storeWord [MemoryInvariantI]:
                         (\<lambda>vAddr. bind (read_state (getPhysicalAddress (vAddr, STORE)))
                         (\<lambda>x. case x of None \<Rightarrow> return True
                                      | Some a' \<Rightarrow> return (a \<notin> Region a' 4)))))) \<and>\<^sub>b
-                  (read_state (getMemData a) =\<^sub>b return val))
+                  (read_state (getMemByte a) =\<^sub>b return val))
                  (storeWord v)
                  (\<lambda>_. read_state getExceptionSignalled \<or>\<^sub>b
                       read_state isUnpredictable \<or>\<^sub>b
-                      read_state (getMemData a) =\<^sub>b return val)"
+                      read_state (getMemByte a) =\<^sub>b return val)"
 unfolding storeWord_alt_def 
 unfolding LegacyStoreVirtualAddress_def getVirtualAddress_alt_def
 unfolding BYTE_def HALFWORD_def WORD_def DOUBLEWORD_def
@@ -1083,11 +1083,11 @@ lemma MemoryInvariant_storeDoubleword [MemoryInvariantI]:
                         (\<lambda>vAddr. bind (read_state (getPhysicalAddress (vAddr, STORE)))
                         (\<lambda>x. case x of None \<Rightarrow> return True
                                      | Some a' \<Rightarrow> return (a \<notin> Region a' 8)))))) \<and>\<^sub>b
-                  (read_state (getMemData a) =\<^sub>b return val))
+                  (read_state (getMemByte a) =\<^sub>b return val))
                  (storeDoubleword v)
                  (\<lambda>_. read_state getExceptionSignalled \<or>\<^sub>b
                       read_state isUnpredictable \<or>\<^sub>b
-                      read_state (getMemData a) =\<^sub>b return val)"
+                      read_state (getMemByte a) =\<^sub>b return val)"
 unfolding storeDoubleword_alt_def 
 unfolding LegacyStoreVirtualAddress_def getVirtualAddress_alt_def
 unfolding BYTE_def HALFWORD_def WORD_def DOUBLEWORD_def
@@ -1096,13 +1096,13 @@ by MemoryInvariant auto?
 (* Code generation - end override *)
 
 lemma MemoryInvariant_dfn'SW [MemoryInvariantI]:
-  shows "PrePost ((read_state (getMemData a) =\<^sub>b return val) \<and>\<^sub>b
+  shows "PrePost ((read_state (getMemByte a) =\<^sub>b return val) \<and>\<^sub>b
                   bind (SWActions v)
                        (\<lambda>p. return (a \<notin> \<Union> (WrittenAddresses ` p))))
                  (dfn'SW v)
                  (\<lambda>_. read_state getExceptionSignalled \<or>\<^sub>b
                       read_state isUnpredictable \<or>\<^sub>b
-                      read_state (getMemData a) =\<^sub>b return val)"
+                      read_state (getMemByte a) =\<^sub>b return val)"
 unfolding dfn'SW_alt_def SWActions_def 
 unfolding LegacyStoreActions_def LegacyStorePhysicalAddress_def LegacyStoreVirtualAddress_def
 unfolding BYTE_def HALFWORD_def WORD_def DOUBLEWORD_def
@@ -1110,13 +1110,13 @@ unfolding CheckBranch_alt_def getVirtualAddress_alt_def
 by MemoryInvariant auto?
 
 lemma MemoryInvariant_dfn'SD [MemoryInvariantI]:
-  shows "PrePost ((read_state (getMemData a) =\<^sub>b return val) \<and>\<^sub>b
+  shows "PrePost ((read_state (getMemByte a) =\<^sub>b return val) \<and>\<^sub>b
                   bind (SDActions v)
                        (\<lambda>p. return (a \<notin> \<Union> (WrittenAddresses ` p))))
                  (dfn'SD v)
                  (\<lambda>_. read_state getExceptionSignalled \<or>\<^sub>b
                       read_state isUnpredictable \<or>\<^sub>b
-                      read_state (getMemData a) =\<^sub>b return val)"
+                      read_state (getMemByte a) =\<^sub>b return val)"
 unfolding dfn'SD_alt_def SDActions_def 
 unfolding LegacyStoreActions_def LegacyStorePhysicalAddress_def LegacyStoreVirtualAddress_def
 unfolding BYTE_def HALFWORD_def WORD_def DOUBLEWORD_def
@@ -1124,13 +1124,13 @@ unfolding CheckBranch_alt_def getVirtualAddress_alt_def
 by MemoryInvariant auto?
 
 lemma MemoryInvariant_dfn'SC [MemoryInvariantI]:
-  shows "PrePost ((read_state (getMemData a) =\<^sub>b return val) \<and>\<^sub>b
+  shows "PrePost ((read_state (getMemByte a) =\<^sub>b return val) \<and>\<^sub>b
                   bind (SCActions v)
                        (\<lambda>p. return (a \<notin> \<Union> (WrittenAddresses ` p))))
                  (dfn'SC v)
                  (\<lambda>_. read_state getExceptionSignalled \<or>\<^sub>b
                       read_state isUnpredictable \<or>\<^sub>b
-                      read_state (getMemData a) =\<^sub>b return val)"
+                      read_state (getMemByte a) =\<^sub>b return val)"
 unfolding dfn'SC_alt_def SCActions_def 
 unfolding LegacyStoreActions_def LegacyStorePhysicalAddress_def LegacyStoreVirtualAddress_def
 unfolding BYTE_def HALFWORD_def WORD_def DOUBLEWORD_def
@@ -1138,13 +1138,13 @@ unfolding CheckBranch_alt_def getVirtualAddress_alt_def
 by MemoryInvariant auto?
 
 lemma MemoryInvariant_dfn'SCD [MemoryInvariantI]:
-  shows "PrePost ((read_state (getMemData a) =\<^sub>b return val) \<and>\<^sub>b
+  shows "PrePost ((read_state (getMemByte a) =\<^sub>b return val) \<and>\<^sub>b
                   bind (SCDActions v)
                        (\<lambda>p. return (a \<notin> \<Union> (WrittenAddresses ` p))))
                  (dfn'SCD v)
                  (\<lambda>_. read_state getExceptionSignalled \<or>\<^sub>b
                       read_state isUnpredictable \<or>\<^sub>b
-                      read_state (getMemData a) =\<^sub>b return val)"
+                      read_state (getMemByte a) =\<^sub>b return val)"
 unfolding dfn'SCD_alt_def SCDActions_def 
 unfolding LegacyStoreActions_def LegacyStorePhysicalAddress_def LegacyStoreVirtualAddress_def
 unfolding BYTE_def HALFWORD_def WORD_def DOUBLEWORD_def
@@ -1154,7 +1154,7 @@ by MemoryInvariant auto?
 (* Code generation - override - dfn'SWL *)
 
 lemma MemoryInvariant_dfn'SWL [MemoryInvariantI]:
-  shows "PrePost ((read_state (getMemData a) =\<^sub>b return val) \<and>\<^sub>b
+  shows "PrePost ((read_state (getMemByte a) =\<^sub>b return val) \<and>\<^sub>b
                   (read_state getCP0ConfigBE) \<and>\<^sub>b
                   (\<not>\<^sub>b read_state getCP0StatusRE) \<and>\<^sub>b
                   bind (SWLActions v)
@@ -1162,7 +1162,7 @@ lemma MemoryInvariant_dfn'SWL [MemoryInvariantI]:
                  (dfn'SWL v)
                  (\<lambda>_. read_state getExceptionSignalled \<or>\<^sub>b
                       read_state isUnpredictable \<or>\<^sub>b
-                      read_state (getMemData a) =\<^sub>b return val)"
+                      read_state (getMemByte a) =\<^sub>b return val)"
 unfolding dfn'SWL_alt_def SWLActions_def 
 unfolding LegacyStoreActions_def LegacyStorePhysicalAddress_def LegacyStoreVirtualAddress_def
 unfolding BYTE_def HALFWORD_def WORD_def DOUBLEWORD_def
@@ -1179,7 +1179,7 @@ by MemoryInvariant
 (* Code generation - override - dfn'SWR *)
 
 lemma MemoryInvariant_dfn'SWR [MemoryInvariantI]:
-  shows "PrePost ((read_state (getMemData a) =\<^sub>b return val) \<and>\<^sub>b
+  shows "PrePost ((read_state (getMemByte a) =\<^sub>b return val) \<and>\<^sub>b
                   (read_state getCP0ConfigBE) \<and>\<^sub>b
                   (\<not>\<^sub>b read_state getCP0StatusRE) \<and>\<^sub>b
                   bind (SWRActions v)
@@ -1187,7 +1187,7 @@ lemma MemoryInvariant_dfn'SWR [MemoryInvariantI]:
                  (dfn'SWR v)
                  (\<lambda>_. read_state getExceptionSignalled \<or>\<^sub>b
                       read_state isUnpredictable \<or>\<^sub>b
-                      read_state (getMemData a) =\<^sub>b return val)"
+                      read_state (getMemByte a) =\<^sub>b return val)"
 proof -
   have [simp]: "x AND - 4 = x AND NOT mask 2" for x :: "'a::len word"
     unfolding word_not_alt max_word_minus mask_def
@@ -1222,7 +1222,7 @@ qed
 (* Code generation - override - dfn'SDL *)
 
 lemma MemoryInvariant_dfn'SDL [MemoryInvariantI]:
-  shows "PrePost ((read_state (getMemData a) =\<^sub>b return val) \<and>\<^sub>b
+  shows "PrePost ((read_state (getMemByte a) =\<^sub>b return val) \<and>\<^sub>b
                   (read_state getCP0ConfigBE) \<and>\<^sub>b
                   (\<not>\<^sub>b read_state getCP0StatusRE) \<and>\<^sub>b
                   bind (SDLActions v)
@@ -1230,7 +1230,7 @@ lemma MemoryInvariant_dfn'SDL [MemoryInvariantI]:
                  (dfn'SDL v)
                  (\<lambda>_. read_state getExceptionSignalled \<or>\<^sub>b
                       read_state isUnpredictable \<or>\<^sub>b
-                      read_state (getMemData a) =\<^sub>b return val)"
+                      read_state (getMemByte a) =\<^sub>b return val)"
 proof -
   have unat_mod_8_less: "unat x mod 8 < n" if "NOT ucast x = y" "unat (NOT y) < n"
   for x :: "64 word" and y :: "3 word" and n
@@ -1268,7 +1268,7 @@ qed
 (* Code generation - override - dfn'SDR *)
 
 lemma MemoryInvariant_dfn'SDR [MemoryInvariantI]:
-  shows "PrePost ((read_state (getMemData a) =\<^sub>b return val) \<and>\<^sub>b
+  shows "PrePost ((read_state (getMemByte a) =\<^sub>b return val) \<and>\<^sub>b
                   (read_state getCP0ConfigBE) \<and>\<^sub>b
                   (\<not>\<^sub>b read_state getCP0StatusRE) \<and>\<^sub>b
                   bind (SDRActions v)
@@ -1276,7 +1276,7 @@ lemma MemoryInvariant_dfn'SDR [MemoryInvariantI]:
                  (dfn'SDR v)
                  (\<lambda>_. read_state getExceptionSignalled \<or>\<^sub>b
                       read_state isUnpredictable \<or>\<^sub>b
-                      read_state (getMemData a) =\<^sub>b return val)"
+                      read_state (getMemByte a) =\<^sub>b return val)"
 proof -
   have [simp]: "x AND - 8 = x AND NOT mask 3" for x :: "'a::len word"
     unfolding word_not_alt max_word_minus mask_def
@@ -1311,228 +1311,228 @@ qed
 (* Code generation - end override *)
 
 lemma MemoryInvariant_dfn'BREAK [MemoryInvariantI]:
-  shows "IsInvariant (read_state (getMemData a) =\<^sub>b return val) dfn'BREAK"
+  shows "IsInvariant (read_state (getMemByte a) =\<^sub>b return val) dfn'BREAK"
 unfolding dfn'BREAK_alt_def 
 by MemoryInvariant auto?
 
 lemma MemoryInvariant_dfn'SYSCALL [MemoryInvariantI]:
-  shows "IsInvariant (read_state (getMemData a) =\<^sub>b return val) dfn'SYSCALL"
+  shows "IsInvariant (read_state (getMemByte a) =\<^sub>b return val) dfn'SYSCALL"
 unfolding dfn'SYSCALL_alt_def 
 by MemoryInvariant auto?
 
 lemma MemoryInvariant_dfn'MTC0 [MemoryInvariantI]:
-  shows "IsInvariant (read_state (getMemData a) =\<^sub>b return val) (dfn'MTC0 v)"
+  shows "IsInvariant (read_state (getMemByte a) =\<^sub>b return val) (dfn'MTC0 v)"
 unfolding dfn'MTC0_alt_def 
 by MemoryInvariant auto?
 
 lemma MemoryInvariant_dfn'DMTC0 [MemoryInvariantI]:
-  shows "IsInvariant (read_state (getMemData a) =\<^sub>b return val) (dfn'DMTC0 v)"
+  shows "IsInvariant (read_state (getMemByte a) =\<^sub>b return val) (dfn'DMTC0 v)"
 unfolding dfn'DMTC0_alt_def 
 by MemoryInvariant auto?
 
 lemma MemoryInvariant_dfn'MFC0 [MemoryInvariantI]:
-  shows "IsInvariant (read_state (getMemData a) =\<^sub>b return val) (dfn'MFC0 v)"
+  shows "IsInvariant (read_state (getMemByte a) =\<^sub>b return val) (dfn'MFC0 v)"
 unfolding dfn'MFC0_alt_def 
 by MemoryInvariant auto?
 
 lemma MemoryInvariant_dfn'DMFC0 [MemoryInvariantI]:
-  shows "IsInvariant (read_state (getMemData a) =\<^sub>b return val) (dfn'DMFC0 v)"
+  shows "IsInvariant (read_state (getMemByte a) =\<^sub>b return val) (dfn'DMFC0 v)"
 unfolding dfn'DMFC0_alt_def 
 by MemoryInvariant auto?
 
 lemma MemoryInvariant_dfn'J [MemoryInvariantI]:
-  shows "IsInvariant (read_state (getMemData a) =\<^sub>b return val) (dfn'J v)"
+  shows "IsInvariant (read_state (getMemByte a) =\<^sub>b return val) (dfn'J v)"
 unfolding dfn'J_alt_def 
 by MemoryInvariant auto?
 
 lemma MemoryInvariant_dfn'JAL [MemoryInvariantI]:
-  shows "IsInvariant (read_state (getMemData a) =\<^sub>b return val) (dfn'JAL v)"
+  shows "IsInvariant (read_state (getMemByte a) =\<^sub>b return val) (dfn'JAL v)"
 unfolding dfn'JAL_alt_def 
 by MemoryInvariant auto?
 
 lemma MemoryInvariant_dfn'JALR [MemoryInvariantI]:
-  shows "IsInvariant (read_state (getMemData a) =\<^sub>b return val) (dfn'JALR v)"
+  shows "IsInvariant (read_state (getMemByte a) =\<^sub>b return val) (dfn'JALR v)"
 unfolding dfn'JALR_alt_def 
 by MemoryInvariant auto?
 
 lemma MemoryInvariant_dfn'JR [MemoryInvariantI]:
-  shows "IsInvariant (read_state (getMemData a) =\<^sub>b return val) (dfn'JR v)"
+  shows "IsInvariant (read_state (getMemByte a) =\<^sub>b return val) (dfn'JR v)"
 unfolding dfn'JR_alt_def 
 by MemoryInvariant auto?
 
 lemma MemoryInvariant_dfn'BEQ [MemoryInvariantI]:
-  shows "IsInvariant (read_state (getMemData a) =\<^sub>b return val) (dfn'BEQ v)"
+  shows "IsInvariant (read_state (getMemByte a) =\<^sub>b return val) (dfn'BEQ v)"
 unfolding dfn'BEQ_alt_def 
 by MemoryInvariant auto?
 
 lemma MemoryInvariant_dfn'BNE [MemoryInvariantI]:
-  shows "IsInvariant (read_state (getMemData a) =\<^sub>b return val) (dfn'BNE v)"
+  shows "IsInvariant (read_state (getMemByte a) =\<^sub>b return val) (dfn'BNE v)"
 unfolding dfn'BNE_alt_def 
 by MemoryInvariant auto?
 
 lemma MemoryInvariant_dfn'BLEZ [MemoryInvariantI]:
-  shows "IsInvariant (read_state (getMemData a) =\<^sub>b return val) (dfn'BLEZ v)"
+  shows "IsInvariant (read_state (getMemByte a) =\<^sub>b return val) (dfn'BLEZ v)"
 unfolding dfn'BLEZ_alt_def 
 by MemoryInvariant auto?
 
 lemma MemoryInvariant_dfn'BGTZ [MemoryInvariantI]:
-  shows "IsInvariant (read_state (getMemData a) =\<^sub>b return val) (dfn'BGTZ v)"
+  shows "IsInvariant (read_state (getMemByte a) =\<^sub>b return val) (dfn'BGTZ v)"
 unfolding dfn'BGTZ_alt_def 
 by MemoryInvariant auto?
 
 lemma MemoryInvariant_dfn'BLTZ [MemoryInvariantI]:
-  shows "IsInvariant (read_state (getMemData a) =\<^sub>b return val) (dfn'BLTZ v)"
+  shows "IsInvariant (read_state (getMemByte a) =\<^sub>b return val) (dfn'BLTZ v)"
 unfolding dfn'BLTZ_alt_def 
 by MemoryInvariant auto?
 
 lemma MemoryInvariant_dfn'BGEZ [MemoryInvariantI]:
-  shows "IsInvariant (read_state (getMemData a) =\<^sub>b return val) (dfn'BGEZ v)"
+  shows "IsInvariant (read_state (getMemByte a) =\<^sub>b return val) (dfn'BGEZ v)"
 unfolding dfn'BGEZ_alt_def 
 by MemoryInvariant auto?
 
 lemma MemoryInvariant_dfn'BLTZAL [MemoryInvariantI]:
-  shows "IsInvariant (read_state (getMemData a) =\<^sub>b return val) (dfn'BLTZAL v)"
+  shows "IsInvariant (read_state (getMemByte a) =\<^sub>b return val) (dfn'BLTZAL v)"
 unfolding dfn'BLTZAL_alt_def 
 by MemoryInvariant auto?
 
 lemma MemoryInvariant_dfn'BGEZAL [MemoryInvariantI]:
-  shows "IsInvariant (read_state (getMemData a) =\<^sub>b return val) (dfn'BGEZAL v)"
+  shows "IsInvariant (read_state (getMemByte a) =\<^sub>b return val) (dfn'BGEZAL v)"
 unfolding dfn'BGEZAL_alt_def 
 by MemoryInvariant auto?
 
 lemma MemoryInvariant_dfn'BEQL [MemoryInvariantI]:
-  shows "IsInvariant (read_state (getMemData a) =\<^sub>b return val) (dfn'BEQL v)"
+  shows "IsInvariant (read_state (getMemByte a) =\<^sub>b return val) (dfn'BEQL v)"
 unfolding dfn'BEQL_alt_def 
 by MemoryInvariant auto?
 
 lemma MemoryInvariant_dfn'BNEL [MemoryInvariantI]:
-  shows "IsInvariant (read_state (getMemData a) =\<^sub>b return val) (dfn'BNEL v)"
+  shows "IsInvariant (read_state (getMemByte a) =\<^sub>b return val) (dfn'BNEL v)"
 unfolding dfn'BNEL_alt_def 
 by MemoryInvariant auto?
 
 lemma MemoryInvariant_dfn'BLEZL [MemoryInvariantI]:
-  shows "IsInvariant (read_state (getMemData a) =\<^sub>b return val) (dfn'BLEZL v)"
+  shows "IsInvariant (read_state (getMemByte a) =\<^sub>b return val) (dfn'BLEZL v)"
 unfolding dfn'BLEZL_alt_def 
 by MemoryInvariant auto?
 
 lemma MemoryInvariant_dfn'BGTZL [MemoryInvariantI]:
-  shows "IsInvariant (read_state (getMemData a) =\<^sub>b return val) (dfn'BGTZL v)"
+  shows "IsInvariant (read_state (getMemByte a) =\<^sub>b return val) (dfn'BGTZL v)"
 unfolding dfn'BGTZL_alt_def 
 by MemoryInvariant auto?
 
 lemma MemoryInvariant_dfn'BLTZL [MemoryInvariantI]:
-  shows "IsInvariant (read_state (getMemData a) =\<^sub>b return val) (dfn'BLTZL v)"
+  shows "IsInvariant (read_state (getMemByte a) =\<^sub>b return val) (dfn'BLTZL v)"
 unfolding dfn'BLTZL_alt_def 
 by MemoryInvariant auto?
 
 lemma MemoryInvariant_dfn'BGEZL [MemoryInvariantI]:
-  shows "IsInvariant (read_state (getMemData a) =\<^sub>b return val) (dfn'BGEZL v)"
+  shows "IsInvariant (read_state (getMemByte a) =\<^sub>b return val) (dfn'BGEZL v)"
 unfolding dfn'BGEZL_alt_def 
 by MemoryInvariant auto?
 
 lemma MemoryInvariant_dfn'BLTZALL [MemoryInvariantI]:
-  shows "IsInvariant (read_state (getMemData a) =\<^sub>b return val) (dfn'BLTZALL v)"
+  shows "IsInvariant (read_state (getMemByte a) =\<^sub>b return val) (dfn'BLTZALL v)"
 unfolding dfn'BLTZALL_alt_def 
 by MemoryInvariant auto?
 
 lemma MemoryInvariant_dfn'BGEZALL [MemoryInvariantI]:
-  shows "IsInvariant (read_state (getMemData a) =\<^sub>b return val) (dfn'BGEZALL v)"
+  shows "IsInvariant (read_state (getMemByte a) =\<^sub>b return val) (dfn'BGEZALL v)"
 unfolding dfn'BGEZALL_alt_def 
 by MemoryInvariant auto?
 
 lemma MemoryInvariant_dfn'RDHWR [MemoryInvariantI]:
-  shows "IsInvariant (read_state (getMemData a) =\<^sub>b return val) (dfn'RDHWR v)"
+  shows "IsInvariant (read_state (getMemByte a) =\<^sub>b return val) (dfn'RDHWR v)"
 unfolding dfn'RDHWR_alt_def 
 by MemoryInvariant auto?
 
 lemma MemoryInvariant_dfn'CACHE [MemoryInvariantI]:
-  shows "IsInvariant (read_state (getMemData a) =\<^sub>b return val) (dfn'CACHE v)"
+  shows "IsInvariant (read_state (getMemByte a) =\<^sub>b return val) (dfn'CACHE v)"
 unfolding dfn'CACHE_alt_def 
 by MemoryInvariant auto?
 
 lemma MemoryInvariant_dfn'ReservedInstruction [MemoryInvariantI]:
-  shows "IsInvariant (read_state (getMemData a) =\<^sub>b return val) dfn'ReservedInstruction"
+  shows "IsInvariant (read_state (getMemByte a) =\<^sub>b return val) dfn'ReservedInstruction"
 unfolding dfn'ReservedInstruction_alt_def 
 by MemoryInvariant auto?
 
 lemma MemoryInvariant_dfn'Unpredictable [MemoryInvariantI]:
-  shows "IsInvariant (read_state (getMemData a) =\<^sub>b return val) dfn'Unpredictable"
+  shows "IsInvariant (read_state (getMemByte a) =\<^sub>b return val) dfn'Unpredictable"
 unfolding dfn'Unpredictable_alt_def 
 by MemoryInvariant auto?
 
 lemma MemoryInvariant_dfn'TLBP [MemoryInvariantI]:
-  shows "IsInvariant (read_state (getMemData a) =\<^sub>b return val) dfn'TLBP"
+  shows "IsInvariant (read_state (getMemByte a) =\<^sub>b return val) dfn'TLBP"
 unfolding dfn'TLBP_alt_def 
 by MemoryInvariant auto?
 
 lemma MemoryInvariant_dfn'TLBR [MemoryInvariantI]:
-  shows "IsInvariant (read_state (getMemData a) =\<^sub>b return val) dfn'TLBR"
+  shows "IsInvariant (read_state (getMemByte a) =\<^sub>b return val) dfn'TLBR"
 unfolding dfn'TLBR_alt_def 
 by MemoryInvariant auto?
 
 lemma MemoryInvariant_dfn'TLBWI [MemoryInvariantI]:
-  shows "IsInvariant (read_state (getMemData a) =\<^sub>b return val) dfn'TLBWI"
+  shows "IsInvariant (read_state (getMemByte a) =\<^sub>b return val) dfn'TLBWI"
 unfolding dfn'TLBWI_alt_def 
 by MemoryInvariant auto?
 
 lemma MemoryInvariant_dfn'TLBWR [MemoryInvariantI]:
-  shows "IsInvariant (read_state (getMemData a) =\<^sub>b return val) dfn'TLBWR"
+  shows "IsInvariant (read_state (getMemByte a) =\<^sub>b return val) dfn'TLBWR"
 unfolding dfn'TLBWR_alt_def 
 by MemoryInvariant auto?
 
 lemma MemoryInvariant_dfn'COP1 [MemoryInvariantI]:
-  shows "IsInvariant (read_state (getMemData a) =\<^sub>b return val) (dfn'COP1 v)"
+  shows "IsInvariant (read_state (getMemByte a) =\<^sub>b return val) (dfn'COP1 v)"
 unfolding dfn'COP1_alt_def 
 by MemoryInvariant auto?
 
 lemma MemoryInvariant_dfn'CGetBase [MemoryInvariantI]:
-  shows "IsInvariant (read_state (getMemData a) =\<^sub>b return val) (dfn'CGetBase v)"
+  shows "IsInvariant (read_state (getMemByte a) =\<^sub>b return val) (dfn'CGetBase v)"
 unfolding dfn'CGetBase_alt_def 
 by MemoryInvariant auto?
 
 lemma MemoryInvariant_dfn'CGetOffset [MemoryInvariantI]:
-  shows "IsInvariant (read_state (getMemData a) =\<^sub>b return val) (dfn'CGetOffset v)"
+  shows "IsInvariant (read_state (getMemByte a) =\<^sub>b return val) (dfn'CGetOffset v)"
 unfolding dfn'CGetOffset_alt_def 
 by MemoryInvariant auto?
 
 lemma MemoryInvariant_dfn'CGetLen [MemoryInvariantI]:
-  shows "IsInvariant (read_state (getMemData a) =\<^sub>b return val) (dfn'CGetLen v)"
+  shows "IsInvariant (read_state (getMemByte a) =\<^sub>b return val) (dfn'CGetLen v)"
 unfolding dfn'CGetLen_alt_def 
 by MemoryInvariant auto?
 
 lemma MemoryInvariant_dfn'CGetTag [MemoryInvariantI]:
-  shows "IsInvariant (read_state (getMemData a) =\<^sub>b return val) (dfn'CGetTag v)"
+  shows "IsInvariant (read_state (getMemByte a) =\<^sub>b return val) (dfn'CGetTag v)"
 unfolding dfn'CGetTag_alt_def 
 by MemoryInvariant auto?
 
 lemma MemoryInvariant_dfn'CGetSealed [MemoryInvariantI]:
-  shows "IsInvariant (read_state (getMemData a) =\<^sub>b return val) (dfn'CGetSealed v)"
+  shows "IsInvariant (read_state (getMemByte a) =\<^sub>b return val) (dfn'CGetSealed v)"
 unfolding dfn'CGetSealed_alt_def 
 by MemoryInvariant auto?
 
 lemma MemoryInvariant_dfn'CGetPerm [MemoryInvariantI]:
-  shows "IsInvariant (read_state (getMemData a) =\<^sub>b return val) (dfn'CGetPerm v)"
+  shows "IsInvariant (read_state (getMemByte a) =\<^sub>b return val) (dfn'CGetPerm v)"
 unfolding dfn'CGetPerm_alt_def 
 by MemoryInvariant auto?
 
 lemma MemoryInvariant_dfn'CGetType [MemoryInvariantI]:
-  shows "IsInvariant (read_state (getMemData a) =\<^sub>b return val) (dfn'CGetType v)"
+  shows "IsInvariant (read_state (getMemByte a) =\<^sub>b return val) (dfn'CGetType v)"
 unfolding dfn'CGetType_alt_def 
 by MemoryInvariant auto?
 
 lemma MemoryInvariant_dfn'CGetAddr [MemoryInvariantI]:
-  shows "IsInvariant (read_state (getMemData a) =\<^sub>b return val) (dfn'CGetAddr v)"
+  shows "IsInvariant (read_state (getMemByte a) =\<^sub>b return val) (dfn'CGetAddr v)"
 unfolding dfn'CGetAddr_alt_def 
 by MemoryInvariant auto?
 
 lemma MemoryInvariant_dfn'CGetPCC [MemoryInvariantI]:
-  shows "PrePost ((read_state (getMemData a) =\<^sub>b return val) \<and>\<^sub>b
+  shows "PrePost ((read_state (getMemByte a) =\<^sub>b return val) \<and>\<^sub>b
                   bind (CGetPCCActions v)
                        (\<lambda>p. return (a \<notin> \<Union> (WrittenAddresses ` p))))
                  (dfn'CGetPCC v)
                  (\<lambda>_. read_state getExceptionSignalled \<or>\<^sub>b
                       read_state isUnpredictable \<or>\<^sub>b
-                      read_state (getMemData a) =\<^sub>b return val)"
+                      read_state (getMemByte a) =\<^sub>b return val)"
 unfolding dfn'CGetPCC_alt_def CGetPCCActions_def 
 unfolding LegacyStoreActions_def LegacyStorePhysicalAddress_def LegacyStoreVirtualAddress_def
 unfolding BYTE_def HALFWORD_def WORD_def DOUBLEWORD_def
@@ -1540,13 +1540,13 @@ unfolding CheckBranch_alt_def getVirtualAddress_alt_def
 by MemoryInvariant auto?
 
 lemma MemoryInvariant_dfn'CGetPCCSetOffset [MemoryInvariantI]:
-  shows "PrePost ((read_state (getMemData a) =\<^sub>b return val) \<and>\<^sub>b
+  shows "PrePost ((read_state (getMemByte a) =\<^sub>b return val) \<and>\<^sub>b
                   bind (CGetPCCSetOffsetActions v)
                        (\<lambda>p. return (a \<notin> \<Union> (WrittenAddresses ` p))))
                  (dfn'CGetPCCSetOffset v)
                  (\<lambda>_. read_state getExceptionSignalled \<or>\<^sub>b
                       read_state isUnpredictable \<or>\<^sub>b
-                      read_state (getMemData a) =\<^sub>b return val)"
+                      read_state (getMemByte a) =\<^sub>b return val)"
 unfolding dfn'CGetPCCSetOffset_alt_def CGetPCCSetOffsetActions_def 
 unfolding LegacyStoreActions_def LegacyStorePhysicalAddress_def LegacyStoreVirtualAddress_def
 unfolding BYTE_def HALFWORD_def WORD_def DOUBLEWORD_def
@@ -1554,23 +1554,23 @@ unfolding CheckBranch_alt_def getVirtualAddress_alt_def
 by MemoryInvariant auto?
 
 lemma MemoryInvariant_dfn'CGetCause [MemoryInvariantI]:
-  shows "IsInvariant (read_state (getMemData a) =\<^sub>b return val) (dfn'CGetCause v)"
+  shows "IsInvariant (read_state (getMemByte a) =\<^sub>b return val) (dfn'CGetCause v)"
 unfolding dfn'CGetCause_alt_def 
 by MemoryInvariant auto?
 
 lemma MemoryInvariant_dfn'CSetCause [MemoryInvariantI]:
-  shows "IsInvariant (read_state (getMemData a) =\<^sub>b return val) (dfn'CSetCause v)"
+  shows "IsInvariant (read_state (getMemByte a) =\<^sub>b return val) (dfn'CSetCause v)"
 unfolding dfn'CSetCause_alt_def 
 by MemoryInvariant auto?
 
 lemma MemoryInvariant_dfn'CIncOffset [MemoryInvariantI]:
-  shows "PrePost ((read_state (getMemData a) =\<^sub>b return val) \<and>\<^sub>b
+  shows "PrePost ((read_state (getMemByte a) =\<^sub>b return val) \<and>\<^sub>b
                   bind (CIncOffsetActions v)
                        (\<lambda>p. return (a \<notin> \<Union> (WrittenAddresses ` p))))
                  (dfn'CIncOffset v)
                  (\<lambda>_. read_state getExceptionSignalled \<or>\<^sub>b
                       read_state isUnpredictable \<or>\<^sub>b
-                      read_state (getMemData a) =\<^sub>b return val)"
+                      read_state (getMemByte a) =\<^sub>b return val)"
 unfolding dfn'CIncOffset_alt_def CIncOffsetActions_def 
 unfolding LegacyStoreActions_def LegacyStorePhysicalAddress_def LegacyStoreVirtualAddress_def
 unfolding BYTE_def HALFWORD_def WORD_def DOUBLEWORD_def
@@ -1578,13 +1578,13 @@ unfolding CheckBranch_alt_def getVirtualAddress_alt_def
 by MemoryInvariant auto?
 
 lemma MemoryInvariant_dfn'CIncOffsetImmediate [MemoryInvariantI]:
-  shows "PrePost ((read_state (getMemData a) =\<^sub>b return val) \<and>\<^sub>b
+  shows "PrePost ((read_state (getMemByte a) =\<^sub>b return val) \<and>\<^sub>b
                   bind (CIncOffsetImmediateActions v)
                        (\<lambda>p. return (a \<notin> \<Union> (WrittenAddresses ` p))))
                  (dfn'CIncOffsetImmediate v)
                  (\<lambda>_. read_state getExceptionSignalled \<or>\<^sub>b
                       read_state isUnpredictable \<or>\<^sub>b
-                      read_state (getMemData a) =\<^sub>b return val)"
+                      read_state (getMemByte a) =\<^sub>b return val)"
 unfolding dfn'CIncOffsetImmediate_alt_def CIncOffsetImmediateActions_def 
 unfolding LegacyStoreActions_def LegacyStorePhysicalAddress_def LegacyStoreVirtualAddress_def
 unfolding BYTE_def HALFWORD_def WORD_def DOUBLEWORD_def
@@ -1592,13 +1592,13 @@ unfolding CheckBranch_alt_def getVirtualAddress_alt_def
 by MemoryInvariant auto?
 
 lemma MemoryInvariant_dfn'CSetBounds [MemoryInvariantI]:
-  shows "PrePost ((read_state (getMemData a) =\<^sub>b return val) \<and>\<^sub>b
+  shows "PrePost ((read_state (getMemByte a) =\<^sub>b return val) \<and>\<^sub>b
                   bind (CSetBoundsActions v)
                        (\<lambda>p. return (a \<notin> \<Union> (WrittenAddresses ` p))))
                  (dfn'CSetBounds v)
                  (\<lambda>_. read_state getExceptionSignalled \<or>\<^sub>b
                       read_state isUnpredictable \<or>\<^sub>b
-                      read_state (getMemData a) =\<^sub>b return val)"
+                      read_state (getMemByte a) =\<^sub>b return val)"
 unfolding dfn'CSetBounds_alt_def CSetBoundsActions_def 
 unfolding LegacyStoreActions_def LegacyStorePhysicalAddress_def LegacyStoreVirtualAddress_def
 unfolding BYTE_def HALFWORD_def WORD_def DOUBLEWORD_def
@@ -1606,13 +1606,13 @@ unfolding CheckBranch_alt_def getVirtualAddress_alt_def
 by MemoryInvariant auto?
 
 lemma MemoryInvariant_dfn'CSetBoundsExact [MemoryInvariantI]:
-  shows "PrePost ((read_state (getMemData a) =\<^sub>b return val) \<and>\<^sub>b
+  shows "PrePost ((read_state (getMemByte a) =\<^sub>b return val) \<and>\<^sub>b
                   bind (CSetBoundsExactActions v)
                        (\<lambda>p. return (a \<notin> \<Union> (WrittenAddresses ` p))))
                  (dfn'CSetBoundsExact v)
                  (\<lambda>_. read_state getExceptionSignalled \<or>\<^sub>b
                       read_state isUnpredictable \<or>\<^sub>b
-                      read_state (getMemData a) =\<^sub>b return val)"
+                      read_state (getMemByte a) =\<^sub>b return val)"
 unfolding dfn'CSetBoundsExact_alt_def CSetBoundsExactActions_def 
 unfolding LegacyStoreActions_def LegacyStorePhysicalAddress_def LegacyStoreVirtualAddress_def
 unfolding BYTE_def HALFWORD_def WORD_def DOUBLEWORD_def
@@ -1620,13 +1620,13 @@ unfolding CheckBranch_alt_def getVirtualAddress_alt_def
 by MemoryInvariant auto?
 
 lemma MemoryInvariant_dfn'CSetBoundsImmediate [MemoryInvariantI]:
-  shows "PrePost ((read_state (getMemData a) =\<^sub>b return val) \<and>\<^sub>b
+  shows "PrePost ((read_state (getMemByte a) =\<^sub>b return val) \<and>\<^sub>b
                   bind (CSetBoundsImmediateActions v)
                        (\<lambda>p. return (a \<notin> \<Union> (WrittenAddresses ` p))))
                  (dfn'CSetBoundsImmediate v)
                  (\<lambda>_. read_state getExceptionSignalled \<or>\<^sub>b
                       read_state isUnpredictable \<or>\<^sub>b
-                      read_state (getMemData a) =\<^sub>b return val)"
+                      read_state (getMemByte a) =\<^sub>b return val)"
 unfolding dfn'CSetBoundsImmediate_alt_def CSetBoundsImmediateActions_def 
 unfolding LegacyStoreActions_def LegacyStorePhysicalAddress_def LegacyStoreVirtualAddress_def
 unfolding BYTE_def HALFWORD_def WORD_def DOUBLEWORD_def
@@ -1634,28 +1634,28 @@ unfolding CheckBranch_alt_def getVirtualAddress_alt_def
 by MemoryInvariant auto?
 
 lemma MemoryInvariant_ClearRegs [MemoryInvariantI]:
-  shows "IsInvariant (read_state (getMemData a) =\<^sub>b return val) (ClearRegs v)"
+  shows "IsInvariant (read_state (getMemByte a) =\<^sub>b return val) (ClearRegs v)"
 unfolding ClearRegs_alt_def 
 by MemoryInvariant auto?
 
 lemma MemoryInvariant_dfn'ClearLo [MemoryInvariantI]:
-  shows "IsInvariant (read_state (getMemData a) =\<^sub>b return val) (dfn'ClearLo v)"
+  shows "IsInvariant (read_state (getMemByte a) =\<^sub>b return val) (dfn'ClearLo v)"
 unfolding dfn'ClearLo_alt_def 
 by MemoryInvariant auto?
 
 lemma MemoryInvariant_dfn'ClearHi [MemoryInvariantI]:
-  shows "IsInvariant (read_state (getMemData a) =\<^sub>b return val) (dfn'ClearHi v)"
+  shows "IsInvariant (read_state (getMemByte a) =\<^sub>b return val) (dfn'ClearHi v)"
 unfolding dfn'ClearHi_alt_def 
 by MemoryInvariant auto?
 
 lemma MemoryInvariant_dfn'CClearLo [MemoryInvariantI]:
-  shows "PrePost ((read_state (getMemData a) =\<^sub>b return val) \<and>\<^sub>b
+  shows "PrePost ((read_state (getMemByte a) =\<^sub>b return val) \<and>\<^sub>b
                   bind (CClearLoActions v)
                        (\<lambda>p. return (a \<notin> \<Union> (WrittenAddresses ` p))))
                  (dfn'CClearLo v)
                  (\<lambda>_. read_state getExceptionSignalled \<or>\<^sub>b
                       read_state isUnpredictable \<or>\<^sub>b
-                      read_state (getMemData a) =\<^sub>b return val)"
+                      read_state (getMemByte a) =\<^sub>b return val)"
 unfolding dfn'CClearLo_alt_def CClearLoActions_def 
 unfolding LegacyStoreActions_def LegacyStorePhysicalAddress_def LegacyStoreVirtualAddress_def
 unfolding BYTE_def HALFWORD_def WORD_def DOUBLEWORD_def
@@ -1663,13 +1663,13 @@ unfolding CheckBranch_alt_def getVirtualAddress_alt_def
 by MemoryInvariant auto?
 
 lemma MemoryInvariant_dfn'CClearHi [MemoryInvariantI]:
-  shows "PrePost ((read_state (getMemData a) =\<^sub>b return val) \<and>\<^sub>b
+  shows "PrePost ((read_state (getMemByte a) =\<^sub>b return val) \<and>\<^sub>b
                   bind (CClearHiActions v)
                        (\<lambda>p. return (a \<notin> \<Union> (WrittenAddresses ` p))))
                  (dfn'CClearHi v)
                  (\<lambda>_. read_state getExceptionSignalled \<or>\<^sub>b
                       read_state isUnpredictable \<or>\<^sub>b
-                      read_state (getMemData a) =\<^sub>b return val)"
+                      read_state (getMemByte a) =\<^sub>b return val)"
 unfolding dfn'CClearHi_alt_def CClearHiActions_def 
 unfolding LegacyStoreActions_def LegacyStorePhysicalAddress_def LegacyStoreVirtualAddress_def
 unfolding BYTE_def HALFWORD_def WORD_def DOUBLEWORD_def
@@ -1677,13 +1677,13 @@ unfolding CheckBranch_alt_def getVirtualAddress_alt_def
 by MemoryInvariant auto?
 
 lemma MemoryInvariant_dfn'CClearTag [MemoryInvariantI]:
-  shows "PrePost ((read_state (getMemData a) =\<^sub>b return val) \<and>\<^sub>b
+  shows "PrePost ((read_state (getMemByte a) =\<^sub>b return val) \<and>\<^sub>b
                   bind (CClearTagActions v)
                        (\<lambda>p. return (a \<notin> \<Union> (WrittenAddresses ` p))))
                  (dfn'CClearTag v)
                  (\<lambda>_. read_state getExceptionSignalled \<or>\<^sub>b
                       read_state isUnpredictable \<or>\<^sub>b
-                      read_state (getMemData a) =\<^sub>b return val)"
+                      read_state (getMemByte a) =\<^sub>b return val)"
 unfolding dfn'CClearTag_alt_def CClearTagActions_def 
 unfolding LegacyStoreActions_def LegacyStorePhysicalAddress_def LegacyStoreVirtualAddress_def
 unfolding BYTE_def HALFWORD_def WORD_def DOUBLEWORD_def
@@ -1691,13 +1691,13 @@ unfolding CheckBranch_alt_def getVirtualAddress_alt_def
 by MemoryInvariant auto?
 
 lemma MemoryInvariant_dfn'CAndPerm [MemoryInvariantI]:
-  shows "PrePost ((read_state (getMemData a) =\<^sub>b return val) \<and>\<^sub>b
+  shows "PrePost ((read_state (getMemByte a) =\<^sub>b return val) \<and>\<^sub>b
                   bind (CAndPermActions v)
                        (\<lambda>p. return (a \<notin> \<Union> (WrittenAddresses ` p))))
                  (dfn'CAndPerm v)
                  (\<lambda>_. read_state getExceptionSignalled \<or>\<^sub>b
                       read_state isUnpredictable \<or>\<^sub>b
-                      read_state (getMemData a) =\<^sub>b return val)"
+                      read_state (getMemByte a) =\<^sub>b return val)"
 unfolding dfn'CAndPerm_alt_def CAndPermActions_def 
 unfolding LegacyStoreActions_def LegacyStorePhysicalAddress_def LegacyStoreVirtualAddress_def
 unfolding BYTE_def HALFWORD_def WORD_def DOUBLEWORD_def
@@ -1705,13 +1705,13 @@ unfolding CheckBranch_alt_def getVirtualAddress_alt_def
 by MemoryInvariant auto?
 
 lemma MemoryInvariant_dfn'CSetOffset [MemoryInvariantI]:
-  shows "PrePost ((read_state (getMemData a) =\<^sub>b return val) \<and>\<^sub>b
+  shows "PrePost ((read_state (getMemByte a) =\<^sub>b return val) \<and>\<^sub>b
                   bind (CSetOffsetActions v)
                        (\<lambda>p. return (a \<notin> \<Union> (WrittenAddresses ` p))))
                  (dfn'CSetOffset v)
                  (\<lambda>_. read_state getExceptionSignalled \<or>\<^sub>b
                       read_state isUnpredictable \<or>\<^sub>b
-                      read_state (getMemData a) =\<^sub>b return val)"
+                      read_state (getMemByte a) =\<^sub>b return val)"
 unfolding dfn'CSetOffset_alt_def CSetOffsetActions_def 
 unfolding LegacyStoreActions_def LegacyStorePhysicalAddress_def LegacyStoreVirtualAddress_def
 unfolding BYTE_def HALFWORD_def WORD_def DOUBLEWORD_def
@@ -1719,28 +1719,28 @@ unfolding CheckBranch_alt_def getVirtualAddress_alt_def
 by MemoryInvariant auto?
 
 lemma MemoryInvariant_dfn'CSub [MemoryInvariantI]:
-  shows "IsInvariant (read_state (getMemData a) =\<^sub>b return val) (dfn'CSub v)"
+  shows "IsInvariant (read_state (getMemByte a) =\<^sub>b return val) (dfn'CSub v)"
 unfolding dfn'CSub_alt_def 
 by MemoryInvariant auto?
 
 lemma MemoryInvariant_dfn'CCheckPerm [MemoryInvariantI]:
-  shows "IsInvariant (read_state (getMemData a) =\<^sub>b return val) (dfn'CCheckPerm v)"
+  shows "IsInvariant (read_state (getMemByte a) =\<^sub>b return val) (dfn'CCheckPerm v)"
 unfolding dfn'CCheckPerm_alt_def 
 by MemoryInvariant auto?
 
 lemma MemoryInvariant_dfn'CCheckType [MemoryInvariantI]:
-  shows "IsInvariant (read_state (getMemData a) =\<^sub>b return val) (dfn'CCheckType v)"
+  shows "IsInvariant (read_state (getMemByte a) =\<^sub>b return val) (dfn'CCheckType v)"
 unfolding dfn'CCheckType_alt_def 
 by MemoryInvariant auto?
 
 lemma MemoryInvariant_dfn'CFromPtr [MemoryInvariantI]:
-  shows "PrePost ((read_state (getMemData a) =\<^sub>b return val) \<and>\<^sub>b
+  shows "PrePost ((read_state (getMemByte a) =\<^sub>b return val) \<and>\<^sub>b
                   bind (CFromPtrActions v)
                        (\<lambda>p. return (a \<notin> \<Union> (WrittenAddresses ` p))))
                  (dfn'CFromPtr v)
                  (\<lambda>_. read_state getExceptionSignalled \<or>\<^sub>b
                       read_state isUnpredictable \<or>\<^sub>b
-                      read_state (getMemData a) =\<^sub>b return val)"
+                      read_state (getMemByte a) =\<^sub>b return val)"
 unfolding dfn'CFromPtr_alt_def CFromPtrActions_def 
 unfolding LegacyStoreActions_def LegacyStorePhysicalAddress_def LegacyStoreVirtualAddress_def
 unfolding BYTE_def HALFWORD_def WORD_def DOUBLEWORD_def
@@ -1748,85 +1748,85 @@ unfolding CheckBranch_alt_def getVirtualAddress_alt_def
 by MemoryInvariant auto?
 
 lemma MemoryInvariant_dfn'CToPtr [MemoryInvariantI]:
-  shows "IsInvariant (read_state (getMemData a) =\<^sub>b return val) (dfn'CToPtr v)"
+  shows "IsInvariant (read_state (getMemByte a) =\<^sub>b return val) (dfn'CToPtr v)"
 unfolding dfn'CToPtr_alt_def 
 by MemoryInvariant auto?
 
 lemma MemoryInvariant_CPtrCmp [MemoryInvariantI]:
-  shows "IsInvariant (read_state (getMemData a) =\<^sub>b return val) (CPtrCmp v)"
+  shows "IsInvariant (read_state (getMemByte a) =\<^sub>b return val) (CPtrCmp v)"
 unfolding CPtrCmp_alt_def 
 by MemoryInvariant auto?
 
 lemma MemoryInvariant_dfn'CEQ [MemoryInvariantI]:
-  shows "IsInvariant (read_state (getMemData a) =\<^sub>b return val) (dfn'CEQ v)"
+  shows "IsInvariant (read_state (getMemByte a) =\<^sub>b return val) (dfn'CEQ v)"
 unfolding dfn'CEQ_alt_def 
 by MemoryInvariant auto?
 
 lemma MemoryInvariant_dfn'CNE [MemoryInvariantI]:
-  shows "IsInvariant (read_state (getMemData a) =\<^sub>b return val) (dfn'CNE v)"
+  shows "IsInvariant (read_state (getMemByte a) =\<^sub>b return val) (dfn'CNE v)"
 unfolding dfn'CNE_alt_def 
 by MemoryInvariant auto?
 
 lemma MemoryInvariant_dfn'CLT [MemoryInvariantI]:
-  shows "IsInvariant (read_state (getMemData a) =\<^sub>b return val) (dfn'CLT v)"
+  shows "IsInvariant (read_state (getMemByte a) =\<^sub>b return val) (dfn'CLT v)"
 unfolding dfn'CLT_alt_def 
 by MemoryInvariant auto?
 
 lemma MemoryInvariant_dfn'CLE [MemoryInvariantI]:
-  shows "IsInvariant (read_state (getMemData a) =\<^sub>b return val) (dfn'CLE v)"
+  shows "IsInvariant (read_state (getMemByte a) =\<^sub>b return val) (dfn'CLE v)"
 unfolding dfn'CLE_alt_def 
 by MemoryInvariant auto?
 
 lemma MemoryInvariant_dfn'CLTU [MemoryInvariantI]:
-  shows "IsInvariant (read_state (getMemData a) =\<^sub>b return val) (dfn'CLTU v)"
+  shows "IsInvariant (read_state (getMemByte a) =\<^sub>b return val) (dfn'CLTU v)"
 unfolding dfn'CLTU_alt_def 
 by MemoryInvariant auto?
 
 lemma MemoryInvariant_dfn'CLEU [MemoryInvariantI]:
-  shows "IsInvariant (read_state (getMemData a) =\<^sub>b return val) (dfn'CLEU v)"
+  shows "IsInvariant (read_state (getMemByte a) =\<^sub>b return val) (dfn'CLEU v)"
 unfolding dfn'CLEU_alt_def 
 by MemoryInvariant auto?
 
 lemma MemoryInvariant_dfn'CEXEQ [MemoryInvariantI]:
-  shows "IsInvariant (read_state (getMemData a) =\<^sub>b return val) (dfn'CEXEQ v)"
+  shows "IsInvariant (read_state (getMemByte a) =\<^sub>b return val) (dfn'CEXEQ v)"
 unfolding dfn'CEXEQ_alt_def 
 by MemoryInvariant auto?
 
 lemma MemoryInvariant_dfn'CNEXEQ [MemoryInvariantI]:
-  shows "IsInvariant (read_state (getMemData a) =\<^sub>b return val) (dfn'CNEXEQ v)"
+  shows "IsInvariant (read_state (getMemByte a) =\<^sub>b return val) (dfn'CNEXEQ v)"
 unfolding dfn'CNEXEQ_alt_def 
 by MemoryInvariant auto?
 
 lemma MemoryInvariant_dfn'CBTU [MemoryInvariantI]:
-  shows "IsInvariant (read_state (getMemData a) =\<^sub>b return val) (dfn'CBTU v)"
+  shows "IsInvariant (read_state (getMemByte a) =\<^sub>b return val) (dfn'CBTU v)"
 unfolding dfn'CBTU_alt_def 
 by MemoryInvariant auto?
 
 lemma MemoryInvariant_dfn'CBTS [MemoryInvariantI]:
-  shows "IsInvariant (read_state (getMemData a) =\<^sub>b return val) (dfn'CBTS v)"
+  shows "IsInvariant (read_state (getMemByte a) =\<^sub>b return val) (dfn'CBTS v)"
 unfolding dfn'CBTS_alt_def 
 by MemoryInvariant auto?
 
 lemma MemoryInvariant_dfn'CBEZ [MemoryInvariantI]:
-  shows "IsInvariant (read_state (getMemData a) =\<^sub>b return val) (dfn'CBEZ v)"
+  shows "IsInvariant (read_state (getMemByte a) =\<^sub>b return val) (dfn'CBEZ v)"
 unfolding dfn'CBEZ_alt_def 
 by MemoryInvariant auto?
 
 lemma MemoryInvariant_dfn'CBNZ [MemoryInvariantI]:
-  shows "IsInvariant (read_state (getMemData a) =\<^sub>b return val) (dfn'CBNZ v)"
+  shows "IsInvariant (read_state (getMemByte a) =\<^sub>b return val) (dfn'CBNZ v)"
 unfolding dfn'CBNZ_alt_def 
 by MemoryInvariant auto?
 
 (* Code generation - override - dfn'CSC *)
 
 lemma MemoryInvariant_dfn'CSC [MemoryInvariantI]:
-  shows "PrePost ((read_state (getMemData a) =\<^sub>b return val) \<and>\<^sub>b
+  shows "PrePost ((read_state (getMemByte a) =\<^sub>b return val) \<and>\<^sub>b
                   bind (CSCActions v)
                        (\<lambda>p. return (a \<notin> \<Union> (WrittenAddresses ` p))))
                  (dfn'CSC v)
                  (\<lambda>_. read_state getExceptionSignalled \<or>\<^sub>b
                       read_state isUnpredictable \<or>\<^sub>b
-                      read_state (getMemData a) =\<^sub>b return val)"
+                      read_state (getMemByte a) =\<^sub>b return val)"
 unfolding dfn'CSC_alt_def CSCActions_def 
 unfolding CSCPhysicalAddress_def CSCVirtualAddress_def
 by MemoryInvariant 
@@ -1836,13 +1836,13 @@ by MemoryInvariant
 (* Code generation - end override *)
 
 lemma MemoryInvariant_dfn'CLC [MemoryInvariantI]:
-  shows "PrePost ((read_state (getMemData a) =\<^sub>b return val) \<and>\<^sub>b
+  shows "PrePost ((read_state (getMemByte a) =\<^sub>b return val) \<and>\<^sub>b
                   bind (CLCActions v)
                        (\<lambda>p. return (a \<notin> \<Union> (WrittenAddresses ` p))))
                  (dfn'CLC v)
                  (\<lambda>_. read_state getExceptionSignalled \<or>\<^sub>b
                       read_state isUnpredictable \<or>\<^sub>b
-                      read_state (getMemData a) =\<^sub>b return val)"
+                      read_state (getMemByte a) =\<^sub>b return val)"
 unfolding dfn'CLC_alt_def CLCActions_def 
 unfolding LegacyStoreActions_def LegacyStorePhysicalAddress_def LegacyStoreVirtualAddress_def
 unfolding BYTE_def HALFWORD_def WORD_def DOUBLEWORD_def
@@ -1850,13 +1850,13 @@ unfolding CheckBranch_alt_def getVirtualAddress_alt_def
 by MemoryInvariant auto?
 
 lemma MemoryInvariant_dfn'CLoad [MemoryInvariantI]:
-  shows "PrePost ((read_state (getMemData a) =\<^sub>b return val) \<and>\<^sub>b
+  shows "PrePost ((read_state (getMemByte a) =\<^sub>b return val) \<and>\<^sub>b
                   bind (CLoadActions v)
                        (\<lambda>p. return (a \<notin> \<Union> (WrittenAddresses ` p))))
                  (dfn'CLoad v)
                  (\<lambda>_. read_state getExceptionSignalled \<or>\<^sub>b
                       read_state isUnpredictable \<or>\<^sub>b
-                      read_state (getMemData a) =\<^sub>b return val)"
+                      read_state (getMemByte a) =\<^sub>b return val)"
 unfolding dfn'CLoad_alt_def CLoadActions_def 
 unfolding LegacyStoreActions_def LegacyStorePhysicalAddress_def LegacyStoreVirtualAddress_def
 unfolding BYTE_def HALFWORD_def WORD_def DOUBLEWORD_def
@@ -1868,13 +1868,13 @@ by MemoryInvariant auto?
 (* Code generation - override - dfn'CStore *)
 
 lemma MemoryInvariant_dfn'CStore [MemoryInvariantI]:
-  shows "PrePost ((read_state (getMemData a) =\<^sub>b return val) \<and>\<^sub>b
+  shows "PrePost ((read_state (getMemByte a) =\<^sub>b return val) \<and>\<^sub>b
                   bind (CStoreActions v)
                        (\<lambda>p. return (a \<notin> \<Union> (WrittenAddresses ` p))))
                  (dfn'CStore v)
                  (\<lambda>_. read_state getExceptionSignalled \<or>\<^sub>b
                       read_state isUnpredictable \<or>\<^sub>b
-                      read_state (getMemData a) =\<^sub>b return val)"
+                      read_state (getMemByte a) =\<^sub>b return val)"
 proof -
   have [simp]: "min (unat x) 3 = unat x" for x :: "2 word"
     using min_unat_length[where 'a=2]
@@ -1890,13 +1890,13 @@ qed
 (* Code generation - end override *)
 
 lemma MemoryInvariant_dfn'CLLC [MemoryInvariantI]:
-  shows "PrePost ((read_state (getMemData a) =\<^sub>b return val) \<and>\<^sub>b
+  shows "PrePost ((read_state (getMemByte a) =\<^sub>b return val) \<and>\<^sub>b
                   bind (CLLCActions v)
                        (\<lambda>p. return (a \<notin> \<Union> (WrittenAddresses ` p))))
                  (dfn'CLLC v)
                  (\<lambda>_. read_state getExceptionSignalled \<or>\<^sub>b
                       read_state isUnpredictable \<or>\<^sub>b
-                      read_state (getMemData a) =\<^sub>b return val)"
+                      read_state (getMemByte a) =\<^sub>b return val)"
 unfolding dfn'CLLC_alt_def CLLCActions_def 
 unfolding LegacyStoreActions_def LegacyStorePhysicalAddress_def LegacyStoreVirtualAddress_def
 unfolding BYTE_def HALFWORD_def WORD_def DOUBLEWORD_def
@@ -1904,13 +1904,13 @@ unfolding CheckBranch_alt_def getVirtualAddress_alt_def
 by MemoryInvariant auto?
 
 lemma MemoryInvariant_dfn'CLLx [MemoryInvariantI]:
-  shows "PrePost ((read_state (getMemData a) =\<^sub>b return val) \<and>\<^sub>b
+  shows "PrePost ((read_state (getMemByte a) =\<^sub>b return val) \<and>\<^sub>b
                   bind (CLLxActions v)
                        (\<lambda>p. return (a \<notin> \<Union> (WrittenAddresses ` p))))
                  (dfn'CLLx v)
                  (\<lambda>_. read_state getExceptionSignalled \<or>\<^sub>b
                       read_state isUnpredictable \<or>\<^sub>b
-                      read_state (getMemData a) =\<^sub>b return val)"
+                      read_state (getMemByte a) =\<^sub>b return val)"
 unfolding dfn'CLLx_alt_def CLLxActions_def 
 unfolding LegacyStoreActions_def LegacyStorePhysicalAddress_def LegacyStoreVirtualAddress_def
 unfolding BYTE_def HALFWORD_def WORD_def DOUBLEWORD_def
@@ -1920,13 +1920,13 @@ by MemoryInvariant auto?
 (* Code generation - override - dfn'CSCC *)
 
 lemma MemoryInvariant_dfn'CSCC [MemoryInvariantI]:
-  shows "PrePost ((read_state (getMemData a) =\<^sub>b return val) \<and>\<^sub>b
+  shows "PrePost ((read_state (getMemByte a) =\<^sub>b return val) \<and>\<^sub>b
                   bind (CSCCActions v)
                        (\<lambda>p. return (a \<notin> \<Union> (WrittenAddresses ` p))))
                  (dfn'CSCC v)
                  (\<lambda>_. read_state getExceptionSignalled \<or>\<^sub>b
                       read_state isUnpredictable \<or>\<^sub>b
-                      read_state (getMemData a) =\<^sub>b return val)"
+                      read_state (getMemByte a) =\<^sub>b return val)"
 unfolding dfn'CSCC_alt_def CSCCActions_def 
 unfolding CSCCPhysicalAddress_def CSCCVirtualAddress_def
 by MemoryInvariant
@@ -1939,13 +1939,13 @@ by MemoryInvariant
 (* Code generation - override - dfn'CSCx *)
 
 lemma MemoryInvariant_dfn'CSCx [MemoryInvariantI]:
-  shows "PrePost ((read_state (getMemData a) =\<^sub>b return val) \<and>\<^sub>b
+  shows "PrePost ((read_state (getMemByte a) =\<^sub>b return val) \<and>\<^sub>b
                   bind (CSCxActions v)
                        (\<lambda>p. return (a \<notin> \<Union> (WrittenAddresses ` p))))
                  (dfn'CSCx v)
                  (\<lambda>_. read_state getExceptionSignalled \<or>\<^sub>b
                       read_state isUnpredictable \<or>\<^sub>b
-                      read_state (getMemData a) =\<^sub>b return val)"
+                      read_state (getMemByte a) =\<^sub>b return val)"
 proof -
   have [simp]: "min (unat x) 3 = unat x" for x :: "2 word"
     using min_unat_length[where 'a=2]
@@ -1961,13 +1961,13 @@ qed
 (* Code generation - end override *)
 
 lemma MemoryInvariant_dfn'CMOVN [MemoryInvariantI]:
-  shows "PrePost ((read_state (getMemData a) =\<^sub>b return val) \<and>\<^sub>b
+  shows "PrePost ((read_state (getMemByte a) =\<^sub>b return val) \<and>\<^sub>b
                   bind (CMOVNActions v)
                        (\<lambda>p. return (a \<notin> \<Union> (WrittenAddresses ` p))))
                  (dfn'CMOVN v)
                  (\<lambda>_. read_state getExceptionSignalled \<or>\<^sub>b
                       read_state isUnpredictable \<or>\<^sub>b
-                      read_state (getMemData a) =\<^sub>b return val)"
+                      read_state (getMemByte a) =\<^sub>b return val)"
 unfolding dfn'CMOVN_alt_def CMOVNActions_def 
 unfolding LegacyStoreActions_def LegacyStorePhysicalAddress_def LegacyStoreVirtualAddress_def
 unfolding BYTE_def HALFWORD_def WORD_def DOUBLEWORD_def
@@ -1975,13 +1975,13 @@ unfolding CheckBranch_alt_def getVirtualAddress_alt_def
 by MemoryInvariant auto?
 
 lemma MemoryInvariant_dfn'CMOVZ [MemoryInvariantI]:
-  shows "PrePost ((read_state (getMemData a) =\<^sub>b return val) \<and>\<^sub>b
+  shows "PrePost ((read_state (getMemByte a) =\<^sub>b return val) \<and>\<^sub>b
                   bind (CMOVZActions v)
                        (\<lambda>p. return (a \<notin> \<Union> (WrittenAddresses ` p))))
                  (dfn'CMOVZ v)
                  (\<lambda>_. read_state getExceptionSignalled \<or>\<^sub>b
                       read_state isUnpredictable \<or>\<^sub>b
-                      read_state (getMemData a) =\<^sub>b return val)"
+                      read_state (getMemByte a) =\<^sub>b return val)"
 unfolding dfn'CMOVZ_alt_def CMOVZActions_def 
 unfolding LegacyStoreActions_def LegacyStorePhysicalAddress_def LegacyStoreVirtualAddress_def
 unfolding BYTE_def HALFWORD_def WORD_def DOUBLEWORD_def
@@ -1989,13 +1989,13 @@ unfolding CheckBranch_alt_def getVirtualAddress_alt_def
 by MemoryInvariant auto?
 
 lemma MemoryInvariant_dfn'CMove [MemoryInvariantI]:
-  shows "PrePost ((read_state (getMemData a) =\<^sub>b return val) \<and>\<^sub>b
+  shows "PrePost ((read_state (getMemByte a) =\<^sub>b return val) \<and>\<^sub>b
                   bind (CMoveActions v)
                        (\<lambda>p. return (a \<notin> \<Union> (WrittenAddresses ` p))))
                  (dfn'CMove v)
                  (\<lambda>_. read_state getExceptionSignalled \<or>\<^sub>b
                       read_state isUnpredictable \<or>\<^sub>b
-                      read_state (getMemData a) =\<^sub>b return val)"
+                      read_state (getMemByte a) =\<^sub>b return val)"
 unfolding dfn'CMove_alt_def CMoveActions_def 
 unfolding LegacyStoreActions_def LegacyStorePhysicalAddress_def LegacyStoreVirtualAddress_def
 unfolding BYTE_def HALFWORD_def WORD_def DOUBLEWORD_def
@@ -2003,18 +2003,18 @@ unfolding CheckBranch_alt_def getVirtualAddress_alt_def
 by MemoryInvariant auto?
 
 lemma MemoryInvariant_dfn'CTestSubset [MemoryInvariantI]:
-  shows "IsInvariant (read_state (getMemData a) =\<^sub>b return val) (dfn'CTestSubset v)"
+  shows "IsInvariant (read_state (getMemByte a) =\<^sub>b return val) (dfn'CTestSubset v)"
 unfolding dfn'CTestSubset_alt_def 
 by MemoryInvariant auto?
 
 lemma MemoryInvariant_dfn'CBuildCap [MemoryInvariantI]:
-  shows "PrePost ((read_state (getMemData a) =\<^sub>b return val) \<and>\<^sub>b
+  shows "PrePost ((read_state (getMemByte a) =\<^sub>b return val) \<and>\<^sub>b
                   bind (CBuildCapActions v)
                        (\<lambda>p. return (a \<notin> \<Union> (WrittenAddresses ` p))))
                  (dfn'CBuildCap v)
                  (\<lambda>_. read_state getExceptionSignalled \<or>\<^sub>b
                       read_state isUnpredictable \<or>\<^sub>b
-                      read_state (getMemData a) =\<^sub>b return val)"
+                      read_state (getMemByte a) =\<^sub>b return val)"
 unfolding dfn'CBuildCap_alt_def CBuildCapActions_def 
 unfolding LegacyStoreActions_def LegacyStorePhysicalAddress_def LegacyStoreVirtualAddress_def
 unfolding BYTE_def HALFWORD_def WORD_def DOUBLEWORD_def
@@ -2022,13 +2022,13 @@ unfolding CheckBranch_alt_def getVirtualAddress_alt_def
 by MemoryInvariant auto?
 
 lemma MemoryInvariant_dfn'CCopyType [MemoryInvariantI]:
-  shows "PrePost ((read_state (getMemData a) =\<^sub>b return val) \<and>\<^sub>b
+  shows "PrePost ((read_state (getMemByte a) =\<^sub>b return val) \<and>\<^sub>b
                   bind (CCopyTypeActions v)
                        (\<lambda>p. return (a \<notin> \<Union> (WrittenAddresses ` p))))
                  (dfn'CCopyType v)
                  (\<lambda>_. read_state getExceptionSignalled \<or>\<^sub>b
                       read_state isUnpredictable \<or>\<^sub>b
-                      read_state (getMemData a) =\<^sub>b return val)"
+                      read_state (getMemByte a) =\<^sub>b return val)"
 unfolding dfn'CCopyType_alt_def CCopyTypeActions_def 
 unfolding LegacyStoreActions_def LegacyStorePhysicalAddress_def LegacyStoreVirtualAddress_def
 unfolding BYTE_def HALFWORD_def WORD_def DOUBLEWORD_def
@@ -2036,13 +2036,13 @@ unfolding CheckBranch_alt_def getVirtualAddress_alt_def
 by MemoryInvariant auto?
 
 lemma MemoryInvariant_dfn'CJR [MemoryInvariantI]:
-  shows "PrePost ((read_state (getMemData a) =\<^sub>b return val) \<and>\<^sub>b
+  shows "PrePost ((read_state (getMemByte a) =\<^sub>b return val) \<and>\<^sub>b
                   bind (CJRActions v)
                        (\<lambda>p. return (a \<notin> \<Union> (WrittenAddresses ` p))))
                  (dfn'CJR v)
                  (\<lambda>_. read_state getExceptionSignalled \<or>\<^sub>b
                       read_state isUnpredictable \<or>\<^sub>b
-                      read_state (getMemData a) =\<^sub>b return val)"
+                      read_state (getMemByte a) =\<^sub>b return val)"
 unfolding dfn'CJR_alt_def CJRActions_def 
 unfolding LegacyStoreActions_def LegacyStorePhysicalAddress_def LegacyStoreVirtualAddress_def
 unfolding BYTE_def HALFWORD_def WORD_def DOUBLEWORD_def
@@ -2050,13 +2050,13 @@ unfolding CheckBranch_alt_def getVirtualAddress_alt_def
 by MemoryInvariant auto?
 
 lemma MemoryInvariant_dfn'CJALR [MemoryInvariantI]:
-  shows "PrePost ((read_state (getMemData a) =\<^sub>b return val) \<and>\<^sub>b
+  shows "PrePost ((read_state (getMemByte a) =\<^sub>b return val) \<and>\<^sub>b
                   bind (CJALRActions v)
                        (\<lambda>p. return (a \<notin> \<Union> (WrittenAddresses ` p))))
                  (dfn'CJALR v)
                  (\<lambda>_. read_state getExceptionSignalled \<or>\<^sub>b
                       read_state isUnpredictable \<or>\<^sub>b
-                      read_state (getMemData a) =\<^sub>b return val)"
+                      read_state (getMemByte a) =\<^sub>b return val)"
 unfolding dfn'CJALR_alt_def CJALRActions_def 
 unfolding LegacyStoreActions_def LegacyStorePhysicalAddress_def LegacyStoreVirtualAddress_def
 unfolding BYTE_def HALFWORD_def WORD_def DOUBLEWORD_def
@@ -2064,13 +2064,13 @@ unfolding CheckBranch_alt_def getVirtualAddress_alt_def
 by MemoryInvariant auto?
 
 lemma MemoryInvariant_dfn'CSeal [MemoryInvariantI]:
-  shows "PrePost ((read_state (getMemData a) =\<^sub>b return val) \<and>\<^sub>b
+  shows "PrePost ((read_state (getMemByte a) =\<^sub>b return val) \<and>\<^sub>b
                   bind (CSealActions v)
                        (\<lambda>p. return (a \<notin> \<Union> (WrittenAddresses ` p))))
                  (dfn'CSeal v)
                  (\<lambda>_. read_state getExceptionSignalled \<or>\<^sub>b
                       read_state isUnpredictable \<or>\<^sub>b
-                      read_state (getMemData a) =\<^sub>b return val)"
+                      read_state (getMemByte a) =\<^sub>b return val)"
 unfolding dfn'CSeal_alt_def CSealActions_def 
 unfolding LegacyStoreActions_def LegacyStorePhysicalAddress_def LegacyStoreVirtualAddress_def
 unfolding BYTE_def HALFWORD_def WORD_def DOUBLEWORD_def
@@ -2078,13 +2078,13 @@ unfolding CheckBranch_alt_def getVirtualAddress_alt_def
 by MemoryInvariant auto?
 
 lemma MemoryInvariant_dfn'CUnseal [MemoryInvariantI]:
-  shows "PrePost ((read_state (getMemData a) =\<^sub>b return val) \<and>\<^sub>b
+  shows "PrePost ((read_state (getMemByte a) =\<^sub>b return val) \<and>\<^sub>b
                   bind (CUnsealActions v)
                        (\<lambda>p. return (a \<notin> \<Union> (WrittenAddresses ` p))))
                  (dfn'CUnseal v)
                  (\<lambda>_. read_state getExceptionSignalled \<or>\<^sub>b
                       read_state isUnpredictable \<or>\<^sub>b
-                      read_state (getMemData a) =\<^sub>b return val)"
+                      read_state (getMemByte a) =\<^sub>b return val)"
 unfolding dfn'CUnseal_alt_def CUnsealActions_def 
 unfolding LegacyStoreActions_def LegacyStorePhysicalAddress_def LegacyStoreVirtualAddress_def
 unfolding BYTE_def HALFWORD_def WORD_def DOUBLEWORD_def
@@ -2092,7 +2092,7 @@ unfolding CheckBranch_alt_def getVirtualAddress_alt_def
 by MemoryInvariant auto?
 
 lemma MemoryInvariant_dfn'CCall [MemoryInvariantI]:
-  shows "IsInvariant (read_state (getMemData a) =\<^sub>b return val) (dfn'CCall v)"
+  shows "IsInvariant (read_state (getMemByte a) =\<^sub>b return val) (dfn'CCall v)"
 unfolding dfn'CCall_alt_def 
 by MemoryInvariant auto?
 
@@ -2105,13 +2105,13 @@ by MemoryInvariant
 (* Code generation - end override *)
 
 lemma MemoryInvariant_dfn'CReadHwr [MemoryInvariantI]:
-  shows "PrePost ((read_state (getMemData a) =\<^sub>b return val) \<and>\<^sub>b
+  shows "PrePost ((read_state (getMemByte a) =\<^sub>b return val) \<and>\<^sub>b
                   bind (CReadHwrActions v)
                        (\<lambda>p. return (a \<notin> \<Union> (WrittenAddresses ` p))))
                  (dfn'CReadHwr v)
                  (\<lambda>_. read_state getExceptionSignalled \<or>\<^sub>b
                       read_state isUnpredictable \<or>\<^sub>b
-                      read_state (getMemData a) =\<^sub>b return val)"
+                      read_state (getMemByte a) =\<^sub>b return val)"
 unfolding dfn'CReadHwr_alt_def CReadHwrActions_def 
 unfolding LegacyStoreActions_def LegacyStorePhysicalAddress_def LegacyStoreVirtualAddress_def
 unfolding BYTE_def HALFWORD_def WORD_def DOUBLEWORD_def
@@ -2119,13 +2119,13 @@ unfolding CheckBranch_alt_def getVirtualAddress_alt_def
 by MemoryInvariant auto?
 
 lemma MemoryInvariant_dfn'CWriteHwr [MemoryInvariantI]:
-  shows "PrePost ((read_state (getMemData a) =\<^sub>b return val) \<and>\<^sub>b
+  shows "PrePost ((read_state (getMemByte a) =\<^sub>b return val) \<and>\<^sub>b
                   bind (CWriteHwrActions v)
                        (\<lambda>p. return (a \<notin> \<Union> (WrittenAddresses ` p))))
                  (dfn'CWriteHwr v)
                  (\<lambda>_. read_state getExceptionSignalled \<or>\<^sub>b
                       read_state isUnpredictable \<or>\<^sub>b
-                      read_state (getMemData a) =\<^sub>b return val)"
+                      read_state (getMemByte a) =\<^sub>b return val)"
 unfolding dfn'CWriteHwr_alt_def CWriteHwrActions_def 
 unfolding LegacyStoreActions_def LegacyStorePhysicalAddress_def LegacyStoreVirtualAddress_def
 unfolding BYTE_def HALFWORD_def WORD_def DOUBLEWORD_def
@@ -2133,19 +2133,19 @@ unfolding CheckBranch_alt_def getVirtualAddress_alt_def
 by MemoryInvariant auto?
 
 lemma MemoryInvariant_dfn'CReturn [MemoryInvariantI]:
-  shows "IsInvariant (read_state (getMemData a) =\<^sub>b return val) dfn'CReturn"
+  shows "IsInvariant (read_state (getMemByte a) =\<^sub>b return val) dfn'CReturn"
 unfolding dfn'CReturn_alt_def 
 by MemoryInvariant auto?
 
 lemma MemoryInvariant_dfn'UnknownCapInstruction [MemoryInvariantI]:
-  shows "IsInvariant (read_state (getMemData a) =\<^sub>b return val) dfn'UnknownCapInstruction"
+  shows "IsInvariant (read_state (getMemByte a) =\<^sub>b return val) dfn'UnknownCapInstruction"
 unfolding dfn'UnknownCapInstruction_alt_def 
 by MemoryInvariant auto?
 
 (* Code generation - override - Run *)
 
 lemma MemoryInvariant_Run_aux:
-  shows "PrePost ((read_state (getMemData a) =\<^sub>b return val) \<and>\<^sub>b
+  shows "PrePost ((read_state (getMemByte a) =\<^sub>b return val) \<and>\<^sub>b
                   (read_state getCP0ConfigBE) \<and>\<^sub>b
                   (\<not>\<^sub>b read_state getCP0StatusRE) \<and>\<^sub>b
                   bind (RunActions v)
@@ -2155,7 +2155,7 @@ lemma MemoryInvariant_Run_aux:
                  (Run v) 
                  (\<lambda>_. read_state getExceptionSignalled \<or>\<^sub>b
                       read_state isUnpredictable \<or>\<^sub>b
-                      read_state (getMemData a) =\<^sub>b return val)"
+                      read_state (getMemByte a) =\<^sub>b return val)"
 unfolding Run_alt_def CheckBranch_alt_def RunActions_def
 by MemoryInvariant auto?
 
@@ -2173,7 +2173,7 @@ unfolding TakeBranch_def
 by PrePost (auto split: option.splits)
 
 lemma MemoryInvariant_Fetch_aux1:
-  shows "IsInvariant ((read_state (getMemData a) =\<^sub>b return val) \<and>\<^sub>b
+  shows "IsInvariant ((read_state (getMemByte a) =\<^sub>b return val) \<and>\<^sub>b
                       (read_state getCP0ConfigBE) \<and>\<^sub>b
                       (\<not>\<^sub>b read_state getCP0StatusRE)) 
                      Fetch"
@@ -2201,7 +2201,7 @@ lemma MemoryInvariant_NextWithGhostState [MemoryInvariantI]:
   shows "PrePost (read_state getEmptyGhostState \<and>\<^sub>b
                   read_state getCP0ConfigBE \<and>\<^sub>b
                   \<not>\<^sub>b read_state getCP0StatusRE \<and>\<^sub>b
-                  (read_state (getMemData a) =\<^sub>b return val) \<and>\<^sub>b
+                  (read_state (getMemByte a) =\<^sub>b return val) \<and>\<^sub>b
                   (read_state CCallFastInstructionParam =\<^sub>b return None) \<and>\<^sub>b
                   bind DomainActions
                        (\<lambda>p. return (\<forall>x\<in>p. a \<notin> WrittenAddresses x)))
@@ -2219,11 +2219,11 @@ theorem MemoryInvariant:
   assumes prov: "a \<notin> \<Union> (WrittenAddresses ` actions)"
       and valid: "getStateIsValid s"
       and suc: "(PreserveDomain actions, s') \<in> NextStates s"
-  shows "getMemData a s' = getMemData a s"
+  shows "getMemByte a s' = getMemByte a s"
 using assms
 using PrePostE[where s=s,
                OF MemoryInvariant_NextWithGhostState
-                  [where a=a and val="getMemData a s"]]
+                  [where a=a and val="getMemByte a s"]]
 unfolding StateIsValid_def
 unfolding NextStates_def Next_NextWithGhostState NextNonExceptionStep_def
 by (auto simp: ValueAndStatePart_simp split: if_splits option.splits)
